examples/formal-languages/regular/charsetScript.sml
@@ -3,6 +3,7 @@ open arithmeticTheory listTheory optionTheory rich_listTheory
      pairTheory comparisonTheory stringTheory;
 
 local open numSyntax Regexp_Type in end;
+
 val comparison_distinct = TypeBase.distinct_of ``:ordering``
 
 val _ = new_theory "charset";
@@ -12,55 +13,56 @@ val _ = new_theory "charset";
 (* Regexp_Type.sml.                                                          *)
 (*---------------------------------------------------------------------------*)
 
-val alphabet_size_def =
- Define
-   `alphabet_size = ^(numSyntax.term_of_int Regexp_Type.alphabet_size)`;
+Definition alphabet_size_def :
+  alphabet_size = ^(numSyntax.term_of_int Regexp_Type.alphabet_size)
+End
 
-val ALPHABET_def =
- Define
-  `ALPHABET = ^(rhs (concl (EVAL ``GENLIST I alphabet_size``)))`;
+Definition ALPHABET_def :
+  ALPHABET = ^(rhs (concl (EVAL ``GENLIST I alphabet_size``)))
+End
 
-val mem_alphabet = Q.store_thm
-("mem_alphabet",
- `!c. MEM c ALPHABET ==> c < alphabet_size`,
- rw_tac std_ss [ALPHABET_def,alphabet_size_def,MEM] >> EVAL_TAC);
+Theorem mem_alphabet :
+ !c. MEM c ALPHABET ==> c < alphabet_size
+Proof
+ rw_tac std_ss [ALPHABET_def,alphabet_size_def,MEM] >> EVAL_TAC
+QED
 
-val alphabet_mem = Q.store_thm
-("alphabet_mem",
- `!c. c < alphabet_size ==> MEM c ALPHABET`,
+Theorem alphabet_mem[local] :
+ !c. c < alphabet_size ==> MEM c ALPHABET
+Proof
  simp_tac bool_ss [alphabet_size_def]
   >> CONV_TAC (REPEATC (numLib.BOUNDED_FORALL_CONV EVAL))
-  >> rw []);
+  >> rw []
+QED
 
-val mem_alphabet_iff = Q.store_thm
-("mem_alphabet_iff",
- `!c. MEM c ALPHABET <=> c < alphabet_size`,
- metis_tac [mem_alphabet,alphabet_mem]);
+Theorem mem_alphabet_iff :
+ !c. MEM c ALPHABET <=> c < alphabet_size
+Proof
+ metis_tac [mem_alphabet,alphabet_mem]
+QED
 
-val ORD_CHR_lem = Q.store_thm
-("ORD_CHR_lem",
- `!c. c < alphabet_size ==> (ORD(CHR c) = c)`,
- rw[alphabet_size_def,GSYM ORD_CHR] >> decide_tac);
+Theorem ORD_CHR_lem :
+ !c. c < alphabet_size ==> (ORD(CHR c) = c)
+Proof
+ rw[alphabet_size_def,GSYM ORD_CHR] >> decide_tac
+QED
 
 
 (*---------------------------------------------------------------------------*)
-(* Charsets are represented by :word64#word64#word64#word64                  *)
+(* Character sets are represented by 4-tuples of word64                      *)
 (*---------------------------------------------------------------------------*)
 
 val _ = Hol_datatype
          `charset = Charset of word64 => word64 => word64 => word64`;
 
-(*---------------------------------------------------------------------------*)
-(* Character sets.                                                           *)
-(*---------------------------------------------------------------------------*)
+Definition charset_empty_def :
+  charset_empty = Charset 0w 0w 0w 0w
+End
 
-val charset_empty_def =
- Define
-   `charset_empty = Charset 0w 0w 0w 0w`;
+Definition charset_full_def :
+   charset_full = Charset (~0w) (~0w) (~0w) (~0w)
+End
 
-val charset_full_def =
- Define
-  `charset_full = Charset (~0w) (~0w) (~0w) (~0w)`;
 
 (*---------------------------------------------------------------------------*)
 (*   |- charset_full =                                                       *)
@@ -69,26 +71,23 @@ val charset_full_def =
 (*         0xFFFFFFFFFFFFFFFFw 0xFFFFFFFFFFFFFFFFw                           *)
 (*---------------------------------------------------------------------------*)
 
-val charset_full_thm = save_thm
-("charset_full_thm",
- CONV_RULE (RHS_CONV EVAL) charset_full_def);
+Theorem charset_full_thm = CONV_RULE (RHS_CONV EVAL) charset_full_def;
 
-val words4_bit_def =
- Define
-   `words4_bit c (Charset w1 w2 w3 w4) =
-       if c < 64 then word_bit c w1 else
-       if c < 128 then word_bit (c-64) w2 else
-       if c < 192 then word_bit (c-128) w3
-       else word_bit (c-192) w4`
-;
+Definition words4_bit_def :
+  words4_bit c (Charset w1 w2 w3 w4) =
+     if c < 128 then
+       (if c < 64 then word_bit c w1 else word_bit (c-64) w2)
+     else
+       (if c < 192 then word_bit (c-128) w3 else word_bit (c-192) w4)
+End
 
-val charset_mem_def =
- Define
-  `charset_mem c (cs:charset) <=> c < alphabet_size /\ words4_bit c cs`;
+Definition charset_mem_def :
+   charset_mem c (cs:charset) <=> c < alphabet_size /\ words4_bit c cs
+End
 
-val charset_union_def =
- Define
-  `charset_union (cs1:charset) (cs2:charset) =
+
+Definition charset_union_def :
+   charset_union (cs1:charset) (cs2:charset) =
     if cs1 = cs2 then cs1 else
     if cs1 = charset_empty then cs2 else
     if cs2 = charset_empty then cs1
@@ -98,27 +97,28 @@ val charset_union_def =
         => Charset (word_or u1 v1)
                    (word_or u2 v2)
                    (word_or u3 v3)
-                   (word_or u4 v4)`
-;
+                   (word_or u4 v4)
+End
 
-val charset_sing_def =
- Define
-  `charset_sing c =
+Definition charset_sing_def :
+   charset_sing c =
      let n = ORD c
      in if n < 64  then Charset (1w << n) 0w 0w 0w else
         if n < 128 then Charset 0w (1w << (n-64)) 0w 0w else
         if n < 192 then Charset 0w 0w (1w << (n-128)) 0w
-        else Charset 0w 0w 0w (1w << (n-192))`
-;
+        else Charset 0w 0w 0w (1w << (n-192))
+End
 
-val charset_insert_def =
- Define
-   `charset_insert c cset = charset_union (charset_sing c) cset`;
+
+Definition charset_insert_def :
+    charset_insert c cset = charset_union (charset_sing c) cset
+End
+
 
 (*
-
-val sanity_check = Q.prove
-(`!c cset. charset_mem (ORD c) (charset_insert c cset)`,
+Theorem sanity_check[local] :
+ !c cset. charset_mem (ORD c) (charset_insert c cset)
+Proof
  rw_tac list_ss [charset_mem_def,charset_insert_def, charset_sing_def,
                  alphabet_size_def,ORD_BOUND,LET_THM]
  >> Cases_on `cset`
@@ -127,14 +127,14 @@ val sanity_check = Q.prove
  >> full_simp_tac list_ss [charset_empty_def]
  >> rw_tac list_ss []
  >> rpt (pop_assum mp_tac)
- >> srw_tac [WORD_ss, WORD_EXTRACT_ss, WORD_BIT_EQ_ss] [])
+ >> srw_tac [WORD_ss, WORD_EXTRACT_ss, WORD_BIT_EQ_ss] []
 
+QED
 *)
 
 
-val charset_cmp_def =
- Define
-  `charset_cmp (Charset u1 u2 u3 u4) (Charset v1 v2 v3 v4) =
+Definition charset_cmp_def :
+   charset_cmp (Charset u1 u2 u3 u4) (Charset v1 v2 v3 v4) =
     case num_cmp (w2n u1) (w2n v1)
       of Less => Less
        | Greater => Greater
@@ -147,23 +147,26 @@ val charset_cmp_def =
       of Less => Less
        | Greater => Greater
        | Equal =>
-    num_cmp (w2n u4) (w2n v4)`
-;
+    num_cmp (w2n u4) (w2n v4)
+End
+
 
 (*---------------------------------------------------------------------------*)
 (* Charset theorems                                                          *)
 (*---------------------------------------------------------------------------*)
 
-val charset_mem_empty = Q.store_thm
-("charset_mem_empty",
- `!c. ~charset_mem c charset_empty`,
+Theorem charset_mem_empty :
+ !c.
+   ~charset_mem c charset_empty
+Proof
   rw_tac list_ss [charset_mem_def,charset_empty_def,words4_bit_def,
-               alphabet_size_def,GSYM IMP_DISJ_THM,wordsTheory.word_bit_0]);
+               alphabet_size_def,GSYM IMP_DISJ_THM,wordsTheory.word_bit_0]
+QED
 
-val charset_mem_union = Q.store_thm
-("charset_mem_union",
- `!c cs1 cs2.
-    charset_mem c (charset_union cs1 cs2) <=> charset_mem c cs1 \/ charset_mem c cs2`,
+Theorem charset_mem_union :
+ !c cs1 cs2.
+    charset_mem c (charset_union cs1 cs2) <=> charset_mem c cs1 \/ charset_mem c cs2
+Proof
  rw_tac list_ss [charset_mem_empty, charset_union_def,EQ_IMP_THM]
   >> REPEAT (WEAKEN_TAC is_neg)
   >> BasicProvers.EVERY_CASE_TAC
@@ -172,21 +175,19 @@ val charset_mem_union = Q.store_thm
   >> full_simp_tac arith_ss []
   >> qpat_x_assum `word_bit _ __` mp_tac
   >> srw_tac [WORD_ss, WORD_EXTRACT_ss, WORD_BIT_EQ_ss] []
-);
+QED
 
-val num_cmp_eq = Q.store_thm
-("num_cmp_eq",
- `!k. num_cmp k k = Equal`,
- rw_tac std_ss [comparisonTheory.num_cmp_def]);
+Theorem num_cmp_eq :
+ !k1 k2.
+   (num_cmp k1 k2 = Equal) <=> (k1 = k2)
+Proof
+ rw_tac std_ss [comparisonTheory.num_cmp_def]
+QED
 
-val charset_cmp_id = Q.store_thm
-("charset_cmp_id",
- `!cs. charset_cmp (cs:charset) cs = Equal`,
- Cases >> rw_tac std_ss [charset_cmp_def,num_cmp_eq]);
-
-val charset_cmp_eq = Q.store_thm
-("charset_cmp_eq",
- `!cs1 cs2. (charset_cmp cs1 cs2 = Equal) <=> (cs1 = cs2)`,
+Theorem charset_cmp_eq :
+ !cs1 cs2.
+   (charset_cmp cs1 cs2 = Equal) <=> (cs1 = cs2)
+Proof
  Cases
   >> Cases
   >> rw_tac std_ss [charset_cmp_def]
@@ -195,50 +196,51 @@ val charset_cmp_eq = Q.store_thm
   >> full_simp_tac std_ss [num_cmp_eq]
   >> rw_tac arith_ss []
   >> rpt (pop_assum mp_tac)
-  >> rw_tac arith_ss [num_cmp_def,wordsTheory.w2n_11]);
+  >> rw_tac arith_ss [num_cmp_def,wordsTheory.w2n_11]
+QED
 
-val charset_cmp_less = Q.prove
-(`!u1 u2 u3 u4 v1 v2 v3 v4.
+Theorem charset_cmp_less[local] :
+ !u1 u2 u3 u4 v1 v2 v3 v4.
     (charset_cmp (Charset u1 u2 u3 u4) (Charset v1 v2 v3 v4) = Less)
    <=>
     w2n u1 < w2n v1
     \/ (w2n u1 = w2n v1) /\ w2n u2 < w2n v2
     \/ (w2n u1 = w2n v1) /\ (w2n u2 = w2n v2) /\ w2n u3 < w2n v3
-    \/ (w2n u1 = w2n v1) /\ (w2n u2 = w2n v2) /\ (w2n u3 = w2n v3) /\ w2n u4 < w2n v4`,
+    \/ (w2n u1 = w2n v1) /\ (w2n u2 = w2n v2) /\ (w2n u3 = w2n v3) /\ w2n u4 < w2n v4
+Proof
   rw_tac std_ss [charset_cmp_def]
   >> BasicProvers.EVERY_CASE_TAC
   >> full_simp_tac std_ss [num_cmp_eq]
   >> rpt (pop_assum mp_tac)
-  >> rw_tac arith_ss [num_cmp_def,wordsTheory.w2n_11]);
+  >> rw_tac arith_ss [num_cmp_def,wordsTheory.w2n_11]
+QED
 
-val charset_cmp_strict = Q.store_thm
-("charset_cmp_strict",
- `!cs1 cs2. (charset_cmp cs1 cs2 = Less) <=> (charset_cmp cs2 cs1 = Greater)`,
- Cases
- >> Cases
+Theorem charset_cmp_strict :
+ !cs1 cs2.
+   (charset_cmp cs1 cs2 = Less) <=> (charset_cmp cs2 cs1 = Greater)
+Proof
+ Cases >> Cases
  >> rw_tac std_ss [charset_cmp_def]
  >> BasicProvers.EVERY_CASE_TAC
  >> metis_tac [num_cmp_good,good_cmp_thm,comparison_distinct])
 ;
 
-val charset_cmp_trans = Q.store_thm
-("charset_cmp_trans",
- `!cs1 cs2 cs3.
+Theorem charset_cmp_trans :
+ !cs1 cs2 cs3.
       (charset_cmp cs1 cs2 = Less) /\
       (charset_cmp cs2 cs3 = Less)
       ==>
-      (charset_cmp cs1 cs3 = Less)`,
-  Cases
-  >> Cases
-  >> Cases
-  >> rw_tac arith_ss [charset_cmp_less]);
+      (charset_cmp cs1 cs3 = Less)
+Proof
+  Cases >> Cases >> Cases
+  >> rw_tac arith_ss [charset_cmp_less]
+QED
 
-val charset_string_def =
- Define
-  `charset_string s =
+Definition charset_string_def :
+   charset_string s =
       FOLDL (\a c. charset_union a (charset_sing c))
             charset_empty
-            s`
-;
+            s
+End
 
 val _ = export_theory();
