examples/formal-languages/regular/regexp_compilerScript.sml
@@ -1,36 +1,108 @@
+(*---------------------------------------------------------------------------*)
+(* Set up context                                                            *)
+(*---------------------------------------------------------------------------*)
+
 open HolKernel Parse boolLib bossLib lcsymtacs numLib;
 open optionTheory pairTheory relationTheory arithmeticTheory
      pred_setTheory bagTheory containerTheory
      listTheory rich_listTheory stringTheory sortingTheory mergesortTheory
-     comparisonTheory balanced_mapTheory eq_cmp_bmapTheory osetTheory
+     comparisonTheory balanced_mapTheory regexp_mapTheory osetTheory
      finite_mapTheory vec_mapTheory charsetTheory regexpTheory
 ;
+
 
 val _ = numLib.prefer_num();
 
 fun pat_elim q = Q.PAT_X_ASSUM q (K ALL_TAC);
 
-val SET_EQ_THM = Q.prove
-(`!s1 s2. (s1 = s2) = !x. s1 x = s2 x`,
- METIS_TAC [EXTENSION,IN_DEF]);
+val byA = BasicProvers.byA;
+infix byA;
 
-val LENGTH_NIL_SYM =
-   GEN_ALL (CONV_RULE (LHS_CONV SYM_CONV) (SPEC_ALL LENGTH_NIL));
+val subst_all_tac = SUBST_ALL_TAC;
+val simp_rule = SIMP_RULE;
+
+val SET_EQ_THM = FUN_EQ_THM;
 
 val list_ss = list_ss ++ rewrites [LENGTH_NIL, LENGTH_NIL_SYM];
 
 val set_ss = list_ss ++ pred_setLib.PRED_SET_ss ++ rewrites [SET_EQ_THM,IN_DEF]
 
-val _ = new_theory "regexp_compiler";
-
 val comparison_distinct = TypeBase.distinct_of ``:ordering``
 
-val eq_cmp_regexp_compare = Q.prove
-(`eq_cmp regexp_compare`,
- metis_tac [eq_cmp_def, regexp_compare_good,regexp_compare_eq]);
+(*---------------------------------------------------------------------------*)
+(* Trivial lemmas                                                            *)
+(*---------------------------------------------------------------------------*)
+
+Triviality INTER_DELETE :
+  !A a. A INTER (A DELETE a) = A DELETE a
+Proof
+  SET_TAC []
+QED
+
+Triviality IN_SET_UNION :
+ !x s t.
+   x IN s ==> (s UNION t = s UNION (x INSERT t))
+Proof
+ SET_TAC []
+QED
+
+Triviality leq_thm :
+  transitive (<=) /\ total (<=) /\ antisymmetric (<=)
+Proof
+   srw_tac [ARITH_ss] [transitive_def, total_def, antisymmetric_def]
+QED
+
+Theorem MAX_LE_THM[local] :
+  !m n. m <= MAX m n /\ n <= MAX m n
+Proof
+  RW_TAC arith_ss [MAX_DEF]
+QED
+
+Theorem IS_SOME_EXISTS[local] :
+  !x. IS_SOME x = ?y. x = SOME y
+Proof
+  Cases THEN METIS_TAC [optionTheory.IS_SOME_DEF]
+QED
+
+Triviality length_mergesort :
+  !l R. LENGTH (mergesort R l) = LENGTH l
+Proof
+  metis_tac[mergesort_perm,PERM_LENGTH]
+QED
+
+Triviality LENGTH_NIL_SYM =
+   GEN_ALL (CONV_RULE (LHS_CONV SYM_CONV) (SPEC_ALL LENGTH_NIL));
+
+Theorem string_to_numlist[local] :
+ !s. (!c. c IN set s ==> ORD c IN set ALPHABET)
+     ==>
+      ?nl. (s = MAP CHR nl) /\
+           (!n. n IN set nl ==> n IN set ALPHABET)
+Proof
+ Induct >> rw []
+  >> `?nl. (s = MAP CHR nl) /\ !n. MEM n nl ==> MEM n ALPHABET` by metis_tac[]
+  >> `?n. (h = CHR n) /\ n < 256` by metis_tac [CHR_ONTO]
+  >> Q.EXISTS_TAC `n::nl`
+  >> rw []
+  >> metis_tac [ORD_CHR_RWT,alphabet_size_def]
+QED
+
+Theorem all_ord_string[local] :
+ EVERY (\c. MEM (ORD c) ALPHABET) s
+   <=>
+  EVERY (\c. ORD c < alphabet_size) s
+Proof
+ simp_tac list_ss [mem_alphabet_iff]
+QED
 
 (*---------------------------------------------------------------------------*)
-(* Output of the compiler is in term of vectors.                             *)
+(* Let's get started                                                         *)
+(*---------------------------------------------------------------------------*)
+
+val _ = new_theory "regexp_compiler";
+
+(*---------------------------------------------------------------------------*)
+(* Output of the compiler is in terms of vectors.                            *)
 (*---------------------------------------------------------------------------*)
 
 val _ = Hol_datatype `vector = Vector of 'a list`;
@@ -44,12 +116,10 @@ End
 Definition length_def : length (Vector l) = LENGTH l
 End
 
-val fromList_Vector = save_thm
-("fromList_Vector",
- SIMP_RULE list_ss [GSYM FUN_EQ_THM] fromList_def);
+Theorem fromList_Vector = SIMP_RULE list_ss [GSYM FUN_EQ_THM] fromList_def;
 
 (*---------------------------------------------------------------------------*)
-(* Manipulate the set of seen states                                         *)
+(* Operations on the set of seen states                                      *)
 (*---------------------------------------------------------------------------*)
 
 val _ = Parse.type_abbrev("regexp_set", ``:(regexp,unit)balanced_map``);
@@ -72,24 +142,113 @@ Definition transitions_def :
   transitions r = MAP (\c. (c,smart_deriv c r)) ALPHABET
 End
 
+(*---------------------------------------------------------------------------*)
+(* Special case for Empty (failure state)                                    *)
+(*---------------------------------------------------------------------------*)
+
+Definition Empty_arcs_def :
+ Empty_arcs =
+  [(0,Empty);  (1,Empty);  (2,Empty);  (3,Empty);
+   (4,Empty);  (5,Empty);  (6,Empty);  (7,Empty);
+   (8,Empty);  (9,Empty);  (10,Empty); (11,Empty);
+   (12,Empty); (13,Empty); (14,Empty); (15,Empty);
+   (16,Empty); (17,Empty); (18,Empty); (19,Empty);
+   (20,Empty); (21,Empty); (22,Empty); (23,Empty);
+   (24,Empty); (25,Empty); (26,Empty); (27,Empty);
+   (28,Empty); (29,Empty); (30,Empty); (31,Empty);
+   (32,Empty); (33,Empty); (34,Empty); (35,Empty);
+   (36,Empty); (37,Empty); (38,Empty); (39,Empty);
+   (40,Empty); (41,Empty); (42,Empty); (43,Empty);
+   (44,Empty); (45,Empty); (46,Empty); (47,Empty);
+   (48,Empty); (49,Empty); (50,Empty); (51,Empty);
+   (52,Empty); (53,Empty); (54,Empty); (55,Empty);
+   (56,Empty); (57,Empty); (58,Empty); (59,Empty);
+   (60,Empty); (61,Empty); (62,Empty); (63,Empty);
+   (64,Empty); (65,Empty); (66,Empty); (67,Empty);
+   (68,Empty); (69,Empty); (70,Empty); (71,Empty);
+   (72,Empty); (73,Empty); (74,Empty); (75,Empty);
+   (76,Empty); (77,Empty); (78,Empty); (79,Empty);
+   (80,Empty); (81,Empty); (82,Empty); (83,Empty);
+   (84,Empty); (85,Empty); (86,Empty); (87,Empty);
+   (88,Empty); (89,Empty); (90,Empty); (91,Empty);
+   (92,Empty); (93,Empty); (94,Empty); (95,Empty);
+   (96,Empty); (97,Empty); (98,Empty); (99,Empty);
+   (100,Empty); (101,Empty) ; (102,Empty); (103,Empty);
+   (104,Empty); (105,Empty);
+   (106,Empty); (107,Empty); (108,Empty); (109,Empty);
+   (110,Empty); (111,Empty); (112,Empty); (113,Empty);
+   (114,Empty); (115,Empty); (116,Empty); (117,Empty);
+   (118,Empty); (119,Empty); (120,Empty); (121,Empty);
+   (122,Empty); (123,Empty); (124,Empty); (125,Empty);
+   (126,Empty); (127,Empty); (128,Empty); (129,Empty);
+   (130,Empty); (131,Empty); (132,Empty); (133,Empty);
+   (134,Empty); (135,Empty); (136,Empty); (137,Empty);
+   (138,Empty); (139,Empty); (140,Empty); (141,Empty);
+   (142,Empty); (143,Empty); (144,Empty); (145,Empty);
+   (146,Empty); (147,Empty); (148,Empty); (149,Empty);
+   (150,Empty); (151,Empty); (152,Empty); (153,Empty);
+   (154,Empty); (155,Empty); (156,Empty); (157,Empty);
+   (158,Empty); (159,Empty); (160,Empty); (161,Empty);
+   (162,Empty); (163,Empty); (164,Empty); (165,Empty);
+   (166,Empty); (167,Empty); (168,Empty); (169,Empty);
+   (170,Empty); (171,Empty); (172,Empty); (173,Empty);
+   (174,Empty); (175,Empty); (176,Empty); (177,Empty);
+   (178,Empty); (179,Empty); (180,Empty); (181,Empty);
+   (182,Empty); (183,Empty); (184,Empty); (185,Empty);
+   (186,Empty); (187,Empty); (188,Empty); (189,Empty);
+   (190,Empty); (191,Empty); (192,Empty); (193,Empty);
+   (194,Empty); (195,Empty); (196,Empty); (197,Empty);
+   (198,Empty); (199,Empty); (200,Empty); (201,Empty);
+   (202,Empty); (203,Empty); (204,Empty); (205,Empty);
+   (206,Empty); (207,Empty); (208,Empty); (209,Empty);
+   (210,Empty); (211,Empty); (212,Empty); (213,Empty);
+   (214,Empty); (215,Empty); (216,Empty); (217,Empty);
+   (218,Empty); (219,Empty); (220,Empty); (221,Empty);
+   (222,Empty); (223,Empty); (224,Empty); (225,Empty);
+   (226,Empty); (227,Empty); (228,Empty); (229,Empty);
+   (230,Empty); (231,Empty); (232,Empty); (233,Empty);
+   (234,Empty); (235,Empty); (236,Empty); (237,Empty);
+   (238,Empty); (239,Empty); (240,Empty); (241,Empty);
+   (242,Empty); (243,Empty); (244,Empty); (245,Empty);
+   (246,Empty); (247,Empty); (248,Empty); (249,Empty);
+   (250,Empty); (251,Empty); (252,Empty); (253,Empty);
+   (254,Empty); (255,Empty)]
+End;
+
+Theorem Empty_arcs_thm :
+  MAP (\c. (c,smart_deriv c Empty)) ALPHABET = Empty_arcs
+Proof
+  rw_tac (srw_ss())
+    [ALPHABET_def, Empty_arcs_def, smart_deriv_def,
+     Empty_def,Epsilon_def,charset_mem_empty]
+QED
+
+Theorem transitions_thm :
+  transitions r = if r = Empty then Empty_arcs
+                  else MAP (\c. (c,smart_deriv c r)) ALPHABET
+Proof
+  rw_tac list_ss [transitions_def] >> metis_tac [Empty_arcs_thm]
+QED
+
 Definition extend_states_def :
  (extend_states next_state state_map trans [] = (next_state,state_map,trans)) /\
  (extend_states next_state state_map trans ((c,r')::t) =
-    case balanced_map$lookup regexp_compare r' state_map
-     of SOME n => extend_states next_state state_map ((c,n)::trans) t
-      | NONE   => extend_states (next_state + 1n)
-                     (balanced_map$insert regexp_compare r' next_state state_map)
-                     ((c,next_state)::trans)
-                     t)
+   case balanced_map$lookup regexp_compare r' state_map
+    of SOME n => extend_states next_state state_map ((c,n)::trans) t
+     | NONE   => extend_states (next_state + 1n)
+                   (balanced_map$insert regexp_compare r' next_state state_map)
+                   ((c,next_state)::trans)
+                   t)
 End
 
 Definition build_table_def :
   build_table arcs r (next_state,state_map,table) =
-    let (next_state,state_map,trans) = extend_states next_state state_map [] arcs
+    let (next_state,state_map,trans) =
+             extend_states next_state state_map [] arcs
     in case balanced_map$lookup regexp_compare r state_map
         of SOME n => (next_state, state_map, (n,trans)::table)
          | NONE   => (next_state + 1n,
-                      balanced_map$insert regexp_compare r next_state state_map,
+                     insert regexp_compare r next_state state_map,
                       (next_state,trans)::table)
 End
 
@@ -100,21 +259,23 @@ End
 (*---------------------------------------------------------------------------*)
 
 Definition Brz_def :
-  Brz seen worklist acc n =
+  Brz seen work acc n =
      if n <= 0n then
        NONE
      else
-     case worklist of
-      | [] => SOME (seen,acc)
-      | r::t =>
-         if mem_regexp r seen then
-             Brz seen t acc (n-1)
-         else
-         let arcs = transitions r
-         in Brz (insert_regexp r seen)
-                (remove_dups (MAP SND arcs) ++ t)
-                (build_table arcs r acc)
-                (n-1)
+     if null work then
+       SOME (seen,acc)
+     else
+         let (m,t) = deleteFindMin work;
+             r = FST m;
+         in if mem_regexp r seen then
+               Brz seen t acc (n-1)
+            else
+             let arcs = transitions r
+             in Brz (insert_regexp r seen)
+                    (FOLDL (\work a. insert_regexp (SND a) work) t arcs)
+                    (build_table arcs r acc)
+                    (n-1)
 End
 
 Definition MAXNUM_32_def :
@@ -125,21 +286,12 @@ End
 (* Build Greve-style Brz function                                            *)
 (*---------------------------------------------------------------------------*)
 
-val MAX_LE_THM = Q.prove
-(`!m n. m <= MAX m n /\ n <= MAX m n`,
- RW_TAC arith_ss [MAX_DEF]);
-
-val IS_SOME_EXISTS = Q.prove
-(`!x. IS_SOME x = ?y. x = SOME y`,
- Cases THEN METIS_TAC [optionTheory.IS_SOME_DEF]);
-
 (*---------------------------------------------------------------------------*)
 (* Domain of the function.                                                   *)
 (*---------------------------------------------------------------------------*)
 
 Definition dom_Brz_def :
- dom_Brz seen worklist acc =
-  ?d. IS_SOME(Brz seen worklist acc d)
+  dom_Brz seen work acc = ?d. IS_SOME(Brz seen work acc d)
 End
 
 (*---------------------------------------------------------------------------*)
@@ -162,14 +314,16 @@ End
 (* well-ordering property.                                                   *)
 (*---------------------------------------------------------------------------*)
 
-val WOP_THM = Q.prove
-(`!P. (?n. P n) ==> ?min. P min /\ !k. P k ==> min <= k`,
- METIS_TAC [arithmeticTheory.WOP,DECIDE ``~(m<n) ==> n<=m``]);
+Theorem WOP_ALT[local] :
+ !P. (?n. P n) ==> ?min. P min /\ !k. P k ==> min <= k
+Proof
+ METIS_TAC [arithmeticTheory.WOP,DECIDE ``~(m<n) ==> n<=m``]
+QED
 
 fun MINCHOOSE (store_name,const_name,tm) =
  let val (V,body) = strip_forall tm
      val P = snd(dest_comb body)
-     val wop_thm = BETA_RULE(SPEC P WOP_THM)
+     val wop_thm = BETA_RULE(SPEC P WOP_ALT)
      val min_term = snd(dest_imp (concl wop_thm))
      val min_term_pred = snd(dest_comb min_term)
      val th1 = BETA_RULE(GSYM (ISPECL [body,min_term_pred] RIGHT_EXISTS_IMP_THM))
@@ -184,15 +338,15 @@ fun MINCHOOSE (store_name,const_name,tm) =
 
 val rdepth_thm =
    MINCHOOSE ("rdepth_thm", "rdepth",
-    ``!seen worklist acc. ?d. IS_SOME(Brz seen worklist acc d)``)
+    ``!seen work acc. ?d. IS_SOME(Brz seen work acc d)``)
 
 (*---------------------------------------------------------------------------*)
 (* Define Brzozo                                                             *)
 (*---------------------------------------------------------------------------*)
 
 Definition Brzozo_def :
-  Brzozo seen worklist acc =
-      THE (Brz seen worklist acc (rdepth seen worklist acc))
+  Brzozo seen work acc =
+      THE (Brz seen work acc (rdepth seen work acc))
 End
 
 
@@ -200,133 +354,171 @@ End
 (* Lemmas about Brz and definedness                                          *)
 (*---------------------------------------------------------------------------*)
 
-val IS_SOME_Brz = Q.prove
-(`!d seen worklist acc.
-      IS_SOME (Brz seen worklist acc d)
-         ==>
-        d <> 0`,
- Cases >> rw[Once Brz_def])
+Theorem IS_SOME_Brz[local] :
+ !d seen work acc.
+    IS_SOME (Brz seen work acc d) ==> d <> 0
+Proof
+ Cases >> rw[Once Brz_def]
+QED
 
-val Brz_SOME = Q.prove
-(`!d seen worklist acc res.
-   (Brz seen worklist acc d = SOME res)
-   ==> d <> 0`,
- METIS_TAC [IS_SOME_Brz,IS_SOME_EXISTS]);
+Theorem Brz_SOME[local] :
+ !d seen work acc res.
+   (Brz seen work acc d = SOME res) ==> d <> 0
+Proof
+ METIS_TAC [IS_SOME_Brz,IS_SOME_EXISTS]
+QED
 
-val Brz_dlem = Q.prove
-(`!d seen worklist acc.
-  IS_SOME (Brz seen worklist acc d)
+Theorem Brz_dlem[local] :
+ !d seen work acc.
+   IS_SOME (Brz seen work acc d)
    ==>
-  (Brz seen worklist acc d = Brz seen worklist acc (SUC d))`,
+   (Brz seen work acc d = Brz seen work acc (SUC d))
+Proof
  Ho_Rewrite.REWRITE_TAC [IS_SOME_EXISTS,GSYM LEFT_FORALL_IMP_THM]
  >> Induct
     >- metis_tac [Brz_SOME]
-    >- (rw[] >> rw[Once Brz_def,LET_THM]
-         >> pop_assum mp_tac
-         >> BasicProvers.EVERY_CASE_TAC
-            >- rw [Brz_def]
-            >- (rw [Once Brz_def] >> metis_tac [])
-            >- (DISCH_THEN (mp_tac o SIMP_RULE list_ss [Once Brz_def])
-                 >> rw[LET_THM]
-                 >> metis_tac[]))
-);
+    >- (rw_tac bool_ss []
+        >> pop_assum (mp_tac o SYM)
+        >> ONCE_REWRITE_TAC [Brz_def]
+        >> rw_tac list_ss [LET_THM]
+        >> Cases_on `(deleteFindMin work)`
+        >> BasicProvers.NORM_TAC list_ss []
+        >> fs[])
+QED
 
-val Brz_monotone = Q.prove
-(`!d1 d2 seen worklist acc.
-      IS_SOME(Brz seen worklist acc d1) /\ d1 <= d2
-       ==> (Brz seen worklist acc d1 = Brz seen worklist acc d2)`,
+Theorem Brz_monotone[local] :
+ !d1 d2 seen work acc.
+      IS_SOME(Brz seen work acc d1) /\ d1 <= d2
+       ==> (Brz seen work acc d1 = Brz seen work acc d2)
+Proof
  RW_TAC arith_ss [LESS_EQ_EXISTS] THEN
- Induct_on `p` THEN METIS_TAC [ADD_CLAUSES,Brz_dlem]);
+ Induct_on `p` THEN METIS_TAC [ADD_CLAUSES,Brz_dlem]
+QED
 
-val Brz_norm = Q.prove
-(`!d seen worklist acc.
-   IS_SOME(Brz seen worklist acc d)
+Theorem Brz_norm[local] :
+ !d seen work acc.
+   IS_SOME(Brz seen work acc d)
     ==>
-   (Brz seen worklist acc d = Brz seen worklist acc (rdepth seen worklist acc))`,
-  METIS_TAC [Brz_monotone,rdepth_thm]);
+   (Brz seen work acc d = Brz seen work acc (rdepth seen work acc))
+Proof
+  METIS_TAC [Brz_monotone,rdepth_thm]
+QED
 
-val Brz_determ = Q.store_thm("Brz_determ",
- `!d1 d2 seen worklist acc.
-    IS_SOME(Brz seen worklist acc d1) /\ IS_SOME(Brz seen worklist acc d2)
-       ==> (Brz seen worklist acc d1 = Brz seen worklist acc d2)`,
-  METIS_TAC [Brz_norm]);
+Theorem Brz_determ :
+ !d1 d2 seen work acc.
+    IS_SOME(Brz seen work acc d1) /\ IS_SOME(Brz seen work acc d2)
+       ==> (Brz seen work acc d1 = Brz seen work acc d2)
+Proof
+  METIS_TAC [Brz_norm]
+QED
 
 (*---------------------------------------------------------------------------*)
 (* Derive eqns for dom_Brz                                                   *)
 (*---------------------------------------------------------------------------*)
 
-val lem = Q.prove
-(`!seen worklist acc.
-   (worklist = []) ==> IS_SOME (Brz seen worklist acc 1)`,
- RW_TAC arith_ss [Once Brz_def]);
+Theorem lem[local] :
+ !seen work acc.
+   null work ==> IS_SOME (Brz seen work acc 1)
+Proof
+ RW_TAC arith_ss [Once Brz_def]
+QED
 
-val dom_base_case = Q.prove
-(`!seen worklist acc.
-   (worklist = []) ==> dom_Brz seen worklist acc`,
- METIS_TAC [dom_Brz_def, lem]);
+Theorem dom_base_case[local] :
+ !seen work acc.
+   null work ==> dom_Brz seen work acc
+Proof
+ METIS_TAC [dom_Brz_def, lem]
+QED
 
-val step2_lem1a = Q.prove
-(`!seen worklist acc r t.
-   (worklist = r::t) /\ mem_regexp r seen /\ dom_Brz seen worklist acc
-    ==> dom_Brz seen t acc`,
- RW_TAC std_ss [dom_Brz_def] THEN
- `d<>0` by METIS_TAC [IS_SOME_Brz] THEN
- Q.EXISTS_TAC `d-1` THEN
- Q.PAT_X_ASSUM `IS_SOME arg` (MP_TAC o ONCE_REWRITE_RULE [Brz_def]) THEN
- CASE_TAC THEN RW_TAC arith_ss [LET_THM]
- THEN METIS_TAC[]);
+Theorem step2_lem1a[local] :
+ !seen work acc r x t.
+   ~null work /\
+   (deleteFindMin work = ((r,x),t)) /\
+   mem_regexp r seen /\ dom_Brz seen work acc
+    ==> dom_Brz seen t acc
+Proof
+ rw_tac std_ss [dom_Brz_def]
+  >> `d<>0` by metis_tac [IS_SOME_Brz]
+  >> qexists_tac `d-1`
+  >> qpat_x_assum `IS_SOME arg` (mp_tac o ONCE_REWRITE_RULE [Brz_def])
+  >> rw_tac arith_ss [LET_THM]
+QED
 
-val step2_lem1b = Q.prove
-(`!seen worklist acc r t arcs.
-   (worklist = r::t) /\ ~mem_regexp r seen /\
-   (arcs = transitions r) /\  dom_Brz seen worklist acc
+Theorem step2_lem1b[local] :
+ !seen work acc r x t arcs.
+   ~null work /\
+   (deleteFindMin work = ((r,x),t)) /\
+   ~mem_regexp r seen /\
+   (arcs = transitions r) /\
+   dom_Brz seen work acc
     ==> dom_Brz (insert_regexp r seen)
-                (remove_dups (MAP SND arcs) ++ t)
-                (build_table arcs r acc)`,
- RW_TAC std_ss [dom_Brz_def] THEN
- `d<>0` by METIS_TAC [IS_SOME_Brz] THEN
- Q.EXISTS_TAC `d-1` THEN
- Q.PAT_X_ASSUM `IS_SOME arg` (MP_TAC o ONCE_REWRITE_RULE [Brz_def]) THEN
- CASE_TAC THEN RW_TAC arith_ss [LET_THM]
- THEN METIS_TAC[]);
+                (FOLDL (\work a. insert_regexp (SND a) work) t arcs)
+                (build_table arcs r acc)
+Proof
+ rw_tac std_ss [dom_Brz_def]
+  >> `d<>0` by metis_tac [IS_SOME_Brz]
+  >> qexists_tac `d-1`
+  >> qpat_x_assum `IS_SOME arg` (mp_tac o ONCE_REWRITE_RULE [Brz_def])
+  >> rw_tac arith_ss [LET_THM]
+QED
 
-val step2_lem2a = Q.prove
-(`!seen worklist acc r t.
-  (worklist = r::t) /\ mem_regexp r seen /\ dom_Brz seen t acc
-   ==> dom_Brz seen worklist acc`,
+Theorem step2_lem2a[local] :
+ !seen work acc r x t.
+   ~null work /\
+   (deleteFindMin work = ((r,x),t)) /\
+   mem_regexp r seen /\ dom_Brz seen t acc
+   ==> dom_Brz seen work acc
+Proof
  rw_tac std_ss [dom_Brz_def]
    >> Q.EXISTS_TAC `SUC d`
-   >> rw [Once Brz_def]);
+   >> rw [Once Brz_def]
+QED
 
-val step2_lem2b = Q.prove
-(`!seen worklist acc r t arcs.
-  (worklist = r::t) /\ (arcs = transitions r) /\
+Theorem step2_lem2b[local] :
+ !seen work acc r x t arcs.
+   ~null work /\
+   (deleteFindMin work = ((r,x),t)) /\
+   (arcs = transitions r) /\
   ~mem_regexp r seen /\
   dom_Brz (insert_regexp r seen)
-          (remove_dups (MAP SND arcs) ++ t)
+          (FOLDL (\work a. insert_regexp (SND a) work) t arcs)
           (build_table arcs r acc)
-   ==> dom_Brz seen worklist acc`,
+   ==> dom_Brz seen work acc
+Proof
  rw_tac std_ss [dom_Brz_def]
    >> Q.EXISTS_TAC `SUC d`
-   >> rw [Once Brz_def,LET_THM]);
+   >> rw [Once Brz_def,LET_THM]
+QED
+
 
 (*---------------------------------------------------------------------------*)
 (* Equational characterization of dom.                                       *)
 (*---------------------------------------------------------------------------*)
 
-val dom_Brz_eqns = Q.store_thm
-("dom_Brz_eqns",
- `(dom_Brz seen [] acc = T) /\
-  (dom_Brz seen (r::t) acc =
-    if mem_regexp r seen
-       then dom_Brz seen t acc
-       else let arcs = transitions r
-            in dom_Brz (insert_regexp r seen)
-                       (remove_dups (MAP SND arcs) ++ t)
-                       (build_table arcs r acc))`,
- CONJ_TAC
-  >- metis_tac [dom_base_case]
-  >- metis_tac [step2_lem1a,step2_lem1b,step2_lem2a,step2_lem2b,LET_THM]);
+Theorem dom_Brz_eqns :
+ dom_Brz seen work acc =
+    if null work then
+      T
+    else let (m,t) = deleteFindMin work ;
+             r = FST m;
+         in
+           if mem_regexp r seen then
+               dom_Brz seen t acc
+           else let arcs = transitions r
+                in dom_Brz (insert_regexp r seen)
+                           (FOLDL (\work a. insert_regexp (SND a) work) t arcs)
+                           (build_table arcs r acc)
+Proof
+ Cases_on `null work`
+  >- metis_tac[dom_base_case]
+  >- (asm_simp_tac list_ss []
+       >> Cases_on `deleteFindMin work`
+       >> rw []
+       >> Cases_on `q`
+       >> fs[]
+          >- metis_tac [step2_lem1a,step2_lem2a]
+          >- metis_tac [step2_lem1b,step2_lem2b])
+QED
 
 (*---------------------------------------------------------------------------*)
 (* Optimization: dom_Brz doesn't depend on its "acc" argument, so can be     *)
@@ -334,116 +526,132 @@ val dom_Brz_eqns = Q.store_thm
 (*---------------------------------------------------------------------------*)
 
 Definition dom_Brz_alt_def :
-  dom_Brz_alt seen worklist = dom_Brz seen worklist ARB
+  dom_Brz_alt seen work = dom_Brz seen work ARB
 End
 
-val acc_irrelevant = Q.prove
-(`!n seen worklist acc acc1.
-     IS_SOME (Brz seen worklist acc n) ==>
-     IS_SOME (Brz seen worklist acc1 n)`,
+Theorem acc_irrelevant[local] :
+ !n seen work acc acc1.
+     IS_SOME (Brz seen work acc n) ==> IS_SOME (Brz seen work acc1 n)
+Proof
  Induct
    >- rw [Once Brz_def]
    >- (ONCE_REWRITE_TAC [Brz_def]
         >> rw_tac list_ss [LET_THM]
-        >> BasicProvers.EVERY_CASE_TAC
-           >- rw []
-           >- metis_tac[]
-           >- metis_tac[]));
+        >> Cases_on `(deleteFindMin work)`
+        >> fs []
+        >> metis_tac[])
+QED
 
-val dom_Brz_alt_equal = Q.store_thm
-("dom_Brz_alt_equal",
- `!seen worklist acc. dom_Brz seen worklist acc = dom_Brz_alt seen worklist`,
- rw [dom_Brz_def, dom_Brz_alt_def] >> metis_tac [acc_irrelevant]);
+Theorem dom_Brz_alt_equal :
+ !seen work acc.
+     dom_Brz seen work acc = dom_Brz_alt seen work
+Proof
+  rw [dom_Brz_def, dom_Brz_alt_def] >> metis_tac [acc_irrelevant]
+QED
 
-
-(*---------------------------------------------------------------------------*)
-(*    |- dom_Brz_alt seen [] /\                                              *)
-(*       (dom_Brz_alt seen (r::t) =                                          *)
-(*         if mem_regexp r seen then                                         *)
-(*            dom_Brz_alt seen t                                             *)
-(*         else                                                              *)
-(*            (let arcs = transitions r                                      *)
-(*             in dom_Brz_alt (insert_regexp r seen)                         *)
-(*                            (remove_dups (MAP SND arcs) ++ t)))            *)
-(*---------------------------------------------------------------------------*)
-
-val dom_Brz_alt_eqns = save_thm
-("dom_Brz_alt_eqns",
- SIMP_RULE bool_ss [dom_Brz_alt_equal] dom_Brz_eqns);
+Theorem dom_Brz_alt_eqns :
+ dom_Brz_alt seen work =
+    if null work then
+      T
+    else let (m,t) = deleteFindMin work ;
+             r = FST m;
+         in
+           if mem_regexp r seen then
+               dom_Brz_alt seen t
+           else let arcs = transitions r
+                in dom_Brz_alt (insert_regexp r seen)
+                           (FOLDL (\work a. insert_regexp (SND a) work) t arcs)
+Proof
+ metis_tac [SIMP_RULE bool_ss [dom_Brz_alt_equal] dom_Brz_eqns]
+QED
 
 (*---------------------------------------------------------------------------*)
 (* Recursion equations for Brzozo                                            *)
 (*---------------------------------------------------------------------------*)
 
-val Brzozo_base = Q.prove
-(`!seen worklist acc.
-    dom_Brz seen worklist acc /\ (worklist = [])
+Theorem Brzozo_base[local] :
+ !seen work acc.
+    dom_Brz seen work acc /\ null work
     ==>
-   (Brzozo seen worklist acc = (seen,acc))`,
- RW_TAC std_ss [Brzozo_def,dom_Brz_def]
-  >> `rdepth seen [] acc <> 0`
+   (Brzozo seen work acc = (seen,acc))
+Proof
+ rw_tac std_ss [Brzozo_def,dom_Brz_def]
+  >> `rdepth seen work acc <> 0`
        by METIS_TAC [IS_SOME_Brz,rdepth_thm]
-  >> RW_TAC arith_ss [Once Brz_def]);
+  >> rw_tac arith_ss [Once Brz_def]
+QED
 
-val Brzozo_rec1 = Q.prove
-(`!seen worklist accr r t.
-    (worklist = r::t) /\
-    dom_Brz seen worklist acc /\
-    mem_regexp r seen
-    ==>
-    (Brzozo seen worklist acc = Brzozo seen t acc)`,
- RW_TAC std_ss [Brzozo_def,dom_Brz_def]
+Theorem Brzozo_rec1[local] :
+ !seen work accr r x t.
+     ~null work /\
+     (deleteFindMin work = ((r,x),t)) /\
+      dom_Brz seen work acc /\
+      mem_regexp r seen
+     ==>
+      (Brzozo seen work acc = Brzozo seen t acc)
+Proof
+ rw_tac std_ss [Brzozo_def,dom_Brz_def]
   >> `d <> 0` by METIS_TAC [IS_SOME_Brz]
-  >> `Brz seen (r::t) acc d = Brz seen t acc (d-1)`
-      by rw_tac list_ss [Once Brz_def]
-  >> METIS_TAC [IS_SOME_EXISTS,NOT_SOME_NONE,THE_DEF,Brz_norm]);
+  >> `Brz seen work acc d = Brz seen t acc (d-1)`
+      by rw_tac list_ss [SimpLHS,Once Brz_def,LET_THM]
+  >> metis_tac [IS_SOME_EXISTS,NOT_SOME_NONE,THE_DEF,Brz_norm]
+QED
 
-val Brzozo_rec2 = Q.prove
-(`!seen worklist accr r t.
-    (worklist = r::t) /\
-    dom_Brz seen worklist acc /\
+Theorem Brzozo_rec2[local] :
+ !seen work accr r x t.
+    ~null work /\
+    (deleteFindMin work = ((r,x),t)) /\
+    dom_Brz seen work acc /\
     ~mem_regexp r seen
     ==>
-    (Brzozo seen worklist acc =
+    (Brzozo seen work acc =
        let arcs = transitions r
        in Brzozo (insert_regexp r seen)
-                 (remove_dups (MAP SND arcs) ++ t)
-                 (build_table arcs r acc))`,
+                 (FOLDL (\work a. insert_regexp (SND a) work) t arcs)
+                 (build_table arcs r acc))
+Proof
  rw_tac std_ss [Brzozo_def,dom_Brz_def,LET_THM]
   >> `d <> 0` by METIS_TAC [IS_SOME_Brz]
-  >> `Brz seen (r::t) acc d =
+  >> `Brz seen work acc d =
       let arcs = transitions r
       in Brz (insert_regexp r seen)
-          (remove_dups (MAP SND arcs) ++ t)
+          (FOLDL (\work a. insert_regexp (SND a) work) t arcs)
           (build_table arcs r acc) (d-1)`
-      by rw_tac list_ss [Once Brz_def,LET_THM]
-  >> METIS_TAC [IS_SOME_EXISTS,NOT_SOME_NONE,THE_DEF,Brz_norm,LET_THM]);
+      by rw_tac list_ss [SimpLHS,Once Brz_def,LET_THM]
+  >> METIS_TAC [IS_SOME_EXISTS,NOT_SOME_NONE,THE_DEF,Brz_norm,LET_THM]
+QED
 
 (*---------------------------------------------------------------------------*)
 (* Equational characterization of Brzozo.                                    *)
 (*---------------------------------------------------------------------------*)
 
-val Brzozo_eqns = Q.prove
-(`!seen worklist acc.
-   dom_Brz seen worklist acc
-  ==>
-   (Brzozo seen worklist acc =
-     case worklist of
-        []  => (seen,acc)
-     | r::t =>
-        if mem_regexp r seen then
-           Brzozo seen t acc
-        else
-          let arcs = transitions r
-          in
-           Brzozo (insert_regexp r seen)
-                  (remove_dups (MAP SND arcs) ++ t)
-                  (build_table arcs r acc))`,
- Cases_on `worklist` >> rpt gen_tac >> CASE_TAC >> rw[LET_THM]
-  >- metis_tac [Brzozo_base]
-  >- metis_tac [Brzozo_rec1]
-  >- metis_tac [Brzozo_rec2]
-);
+Theorem Brzozo_eqns[local] :
+ !seen work acc.
+    dom_Brz seen work acc
+    ==>
+     Brzozo seen work acc =
+       if null work then
+          (seen,acc)
+       else
+         let (rp,t) = deleteFindMin work;
+                  r = FST rp;
+         in
+           if mem_regexp r seen then
+              Brzozo seen t acc
+          else
+            let arcs = transitions r
+            in
+             Brzozo (insert_regexp r seen)
+                    (FOLDL (\work a. insert_regexp (SND a) work) t arcs)
+                    (build_table arcs r acc)
+Proof
+ rw_tac list_ss [LET_THM]
+ >- metis_tac [Brzozo_base]
+ >- (Cases_on `deleteFindMin work`
+      >> Cases_on `q`
+      >> fs[]
+      >> metis_tac [Brzozo_rec1,Brzozo_rec2])
+QED
 
 (*---------------------------------------------------------------------------*)
 (* Now prove induction theorem. This is based on using rdepth as a measure   *)
@@ -451,137 +659,168 @@ val Brzozo_eqns = Q.prove
 (* decreases in recursive calls.                                             *)
 (*---------------------------------------------------------------------------*)
 
-val step3a_lt = Q.prove
-(`!seen worklist acc r t.
-    (worklist = r::t) /\ mem_regexp r seen /\
-    dom_Brz seen worklist acc
-    ==> rdepth seen t acc  < rdepth seen worklist acc`,
+Theorem step3a_lt[local] :
+ !seen work acc r x t.
+   ~null work /\
+   (deleteFindMin work = ((r,x),t)) /\
+   mem_regexp r seen /\
+    dom_Brz seen work acc
+    ==> rdepth seen t acc  < rdepth seen work acc
+Proof
  rw_tac std_ss [dom_Brz_def] THEN IMP_RES_TAC rdepth_thm THEN
-   `rdepth seen (r::t) acc <> 0` by METIS_TAC [IS_SOME_Brz] THEN
-   `rdepth seen (r::t) acc - 1 < rdepth seen (r::t) acc` by DECIDE_TAC THEN
-   `IS_SOME (Brz seen t acc (rdepth seen (r::t) acc - 1))`
-     by (Q.PAT_X_ASSUM `IS_SOME (Brz seen (r::t) acc (rdepth seen (r::t) acc))`
-          (mp_tac o SIMP_RULE arith_ss [Once Brz_def])
-        >> CASE_TAC >> rw[LET_THM]
-           >- metis_tac[]
-           >- metis_tac[])
-    >> `rdepth seen t acc <= rdepth seen (r::t) acc - 1`
+   `rdepth seen work acc <> 0` by METIS_TAC [IS_SOME_Brz] THEN
+   `rdepth seen work acc - 1 < rdepth seen work acc` by DECIDE_TAC THEN
+   `IS_SOME (Brz seen t acc (rdepth seen work acc - 1))`
+     by (qpat_x_assum `IS_SOME (Brz seen work acc (rdepth seen work acc))`
+              (mp_tac o SIMP_RULE arith_ss [Once Brz_def])
+         >> rw[LET_THM])
+    >> `rdepth seen t acc <= rdepth seen work acc - 1`
         by metis_tac [rdepth_thm]
-    >> decide_tac);
+    >> decide_tac
+QED
 
-val step3b_lt = Q.prove
-(`!seen worklist acc r t arcs.
-    (worklist = r::t) /\ ~mem_regexp r seen /\
-    (arcs = transitions r) /\ dom_Brz seen worklist acc
+Theorem step3b_lt[local] :
+ !seen work acc r x t arcs.
+    ~null work /\
+    (deleteFindMin work = ((r,x),t)) /\
+    ~mem_regexp r seen /\
+    (arcs = transitions r) /\ dom_Brz seen work acc
     ==> rdepth (insert_regexp r seen)
-               (remove_dups (MAP SND arcs) ++ t)
-               (build_table arcs r acc)  < rdepth seen worklist acc`,
+               (FOLDL (\work a. insert_regexp (SND a) work) t arcs)
+               (build_table arcs r acc)
+         <
+        rdepth seen work acc
+Proof
  rw_tac std_ss [dom_Brz_def] THEN IMP_RES_TAC rdepth_thm
-  >> `rdepth seen (r::t) acc <> 0` by METIS_TAC [IS_SOME_Brz]
-  >> `rdepth seen (r::t) acc - 1 < rdepth seen (r::t) acc` by DECIDE_TAC
+  >> `rdepth seen work acc <> 0` by METIS_TAC [IS_SOME_Brz]
+  >> `rdepth seen work acc - 1 < rdepth seen work acc` by DECIDE_TAC
   >> `IS_SOME (Brz (insert_regexp r seen)
-                   (remove_dups (MAP SND (transitions r)) ++ t)
+                   (FOLDL (\work a. insert_regexp (SND a) work) t (transitions r))
                    (build_table (transitions r) r acc)
-                   (rdepth seen (r::t) acc - 1))`
-     by (Q.PAT_X_ASSUM `IS_SOME (Brz seen (r::t) acc (rdepth seen (r::t) acc))`
-          (mp_tac o SIMP_RULE arith_ss [Once Brz_def])
-        >> CASE_TAC >> rw[LET_THM]
-           >- metis_tac[]
-           >- metis_tac[])
+                   (rdepth seen work acc - 1))`
+     by (qpat_x_assum `IS_SOME (Brz seen work acc (rdepth seen work acc))`
+              (mp_tac o SIMP_RULE arith_ss [Once Brz_def])
+         >> rw[LET_THM])
     >> `rdepth (insert_regexp r seen)
-               (remove_dups (MAP SND (transitions r)) ++ t)
-               (build_table (transitions r) r acc) <= rdepth seen (r::t) acc - 1`
+               (FOLDL (\work a. insert_regexp (SND a) work) t (transitions r))
+               (build_table (transitions r) r acc) <= rdepth seen work acc - 1`
         by metis_tac [rdepth_thm]
-    >> decide_tac);
+    >> decide_tac
+QED
 
 (*---------------------------------------------------------------------------*)
 (* Induction for Brzozo is obtained by instantiating the WF induction        *)
 (* theorem with the rdepth measure and then simplifying.                     *)
 (*---------------------------------------------------------------------------*)
 
-val ind0 = MATCH_MP relationTheory.WF_INDUCTION_THM
-                    (Q.ISPEC `\(seen,worklist,acc). rdepth seen worklist acc`
-                             prim_recTheory.WF_measure);
-val ind1 = SIMP_RULE std_ss [prim_recTheory.measure_thm] ind0;
-val ind2 = SIMP_RULE std_ss [pairTheory.FORALL_PROD]
-      (Q.ISPEC `\(seen,worklist,acc).
-                    dom_Brz seen worklist acc ==> P seen worklist acc` ind1);
-val ind3 = Q.prove
-(`!P. (!seen worklist acc.
-         (!a b c. rdepth a b c < rdepth seen worklist acc
+Theorem ind_lemA =
+  prim_recTheory.WF_measure
+   |> Q.ISPEC `\(seen,work,acc). rdepth seen work acc`
+   |> MATCH_MP relationTheory.WF_INDUCTION_THM
+   |> simp_rule std_ss [prim_recTheory.measure_thm]
+   |> Q.ISPEC `\(seen,work,acc).
+                  dom_Brz seen work acc ==> P seen work acc`
+   |> simp_rule std_ss [pairTheory.FORALL_PROD]
+;
+
+Theorem ind_lemB[local] :
+  !P. (!seen work acc.
+         (!a b c. rdepth a b c < rdepth seen work acc
                   ==> dom_Brz a b c
                   ==> P a b c)
-         ==> dom_Brz seen worklist acc ==> P seen worklist acc)
+         ==> dom_Brz seen work acc ==> P seen work acc)
   ==>
-  !seen worklist acc. dom_Brz seen worklist acc ==> P seen worklist acc`,
+  !seen work acc. dom_Brz seen work acc ==> P seen work acc
+Proof
 rpt strip_tac
  >> pop_assum mp_tac
- >> Cases_on `acc`
- >> Cases_on `r`
- >> Q.SPEC_TAC (`r'`,`w`)
- >> Q.SPEC_TAC (`q'`,`v`)
- >> Q.SPEC_TAC (`q`,`u`)
- >> Q.ID_SPEC_TAC `worklist`
- >> Q.ID_SPEC_TAC `seen`
- >> match_mp_tac ind2
- >> fs [FORALL_PROD]);
+ >> `?a b c. acc = (a,b,c)` by metis_tac [ABS_PAIR_THM]
+ >> pop_assum SUBST_ALL_TAC
+ >> MAP_EVERY Q.ID_SPEC_TAC [`a`,`b`, `c`,`work`,`seen`]
+ >> match_mp_tac ind_lemA
+ >> fs [FORALL_PROD]
+QED
 
-val Brzozowski_ind = Q.store_thm
-("Brzozowski_ind",
- `!P.
-   (!seen worklist acc.
-       dom_Brz seen worklist acc /\
-       (!r t. (worklist = r::t) /\ mem_regexp r seen ==> P seen t acc) /\
-       (!r t arcs. (arcs = transitions r) /\ (worklist = r::t) /\ ~mem_regexp r seen
-                   ==> P (insert_regexp r seen)
-                         (remove_dups (MAP SND arcs) ++ t)
-                         (build_table arcs r acc))
-         ==> P seen worklist acc)
-  ==> !seen worklist acc. dom_Brz seen worklist acc ==> P seen worklist acc`,
-  gen_tac >> strip_tac
-  >> HO_MATCH_MP_TAC ind3
-  >> rw[]
-  >> metis_tac [step3a_lt,step3b_lt,dom_Brz_eqns]);
+Theorem Brzozowski_ind :
+ !P.
+   (!seen work acc.
+       dom_Brz seen work acc /\
+       (!r x t. ~null work /\
+                (deleteFindMin work = ((r,x),t)) /\
+                mem_regexp r seen ==> P seen t acc) /\
+       (!r x t arcs.
+           ~null work /\ (deleteFindMin work = ((r,x),t)) /\
+           (arcs = transitions r) /\ ~mem_regexp r seen
+           ==> P (insert_regexp r seen)
+                 (FOLDL (\work a. insert_regexp (SND a) work) t arcs)
+                 (build_table arcs r acc))
+         ==> P seen work acc)
+  ==> !seen work acc. dom_Brz seen work acc ==> P seen work acc
+Proof
+  gen_tac
+  >> strip_tac
+  >> ho_match_mp_tac ind_lemB
+  >> simp_tac bool_ss [AND_IMP_INTRO]
+  >> rpt gen_tac
+  >> disch_then (fn th => first_x_assum match_mp_tac >> assume_tac th)
+  >> rw []
+  >> (first_x_assum match_mp_tac
+       >> asm_simp_tac list_ss [step3a_lt,step3b_lt]
+       >> mp_tac dom_Brz_eqns
+       >> rw [])
+QED
 
 (*---------------------------------------------------------------------------*)
 (* Efficient executable version of Brzozo                                    *)
 (*---------------------------------------------------------------------------*)
 
 Definition exec_Brz_def :
-  exec_Brz seen worklist acc d =
+  exec_Brz seen work acc d =
     if d=0n then
-       (if dom_Brz seen worklist acc then Brzozo seen worklist acc else ARB)
+       (if dom_Brz seen work acc then Brzozo seen work acc else ARB)
     else
-      case worklist
-       of [] => (seen,acc)
-       | r::t =>
+    if null work then
+          (seen,acc)
+    else
+      let (m,t) = deleteFindMin work ;
+              r = FST m;
+      in
          if mem_regexp r seen then
              exec_Brz seen t acc (d - 1)
-           else
-             let arcs = transitions r
-             in exec_Brz (insert_regexp r seen)
-                         (remove_dups (MAP SND arcs) ++ t)
-                         (build_table arcs r acc) (d - 1)
+         else
+           let arcs = transitions r
+           in exec_Brz (insert_regexp r seen)
+                       (FOLDL (\work a. insert_regexp (SND a) work) t arcs)
+                       (build_table arcs r acc) (d - 1)
 End
 
-val exec_Brz_equals_Brzozo = Q.prove
-(`!d seen worklist acc.
-    dom_Brz seen worklist acc
-   ==>
-    (exec_Brz seen worklist acc d = Brzozo seen worklist acc)`,
+Theorem exec_Brz_equals_Brzozo[local] :
+  !d seen work acc.
+    dom_Brz seen work acc
+    ==>
+     (exec_Brz seen work acc d = Brzozo seen work acc)
+Proof
  Induct
   >> rw_tac std_ss [Once exec_Brz_def,LET_THM]
-  >> pop_assum mp_tac
-  >> CASE_TAC
-    >- rw [Brzozo_eqns,dom_Brz_eqns]
-    >- rw [Brzozo_eqns,dom_Brz_eqns,LET_THM]);
+  >- metis_tac [Brzozo_eqns]
+  >- (`?r x t. deleteFindMin work = ((r,x),t)` by metis_tac [ABS_PAIR_THM]
+      >> rw [Brzozo_eqns]
+      >> (first_x_assum match_mp_tac
+           >> qpat_x_assum `dom_Brz seen work acc`
+              (mp_tac o SIMP_RULE list_ss [Once dom_Brz_eqns])
+           >> rw []))
+QED
+
+(*---------------------------------------------------------------------------*)
+(* The final definition of the core functionality of the compiler            *)
+(*---------------------------------------------------------------------------*)
 
 Definition Brzozowski_def :
-  Brzozowski seen worklist acc =
-      if dom_Brz seen worklist acc then
-         Brzozo seen worklist acc
+  Brzozowski seen work acc =
+      if dom_Brz seen work acc then
+         Brzozo seen work acc
       else
-         exec_Brz seen worklist acc MAXNUM_32
+         exec_Brz seen work acc MAXNUM_32
 End
 
 (*---------------------------------------------------------------------------*)
@@ -589,38 +828,45 @@ End
 (* In order to evaluate Brzozowski, we can dispatch to exec_Brz.             *)
 (*---------------------------------------------------------------------------*)
 
-val Brzozowski_exec_Brz = Q.store_thm
-("Brzozowski_exec_Brz",
- `Brzozowski seen worklist acc = exec_Brz seen worklist acc MAXNUM_32`,
- rw_tac std_ss [Brzozowski_def,exec_Brz_equals_Brzozo]);
+Theorem Brzozowski_exec_Brz :
+   Brzozowski seen work acc = exec_Brz seen work acc MAXNUM_32
+Proof
+ rw_tac std_ss [Brzozowski_def,exec_Brz_equals_Brzozo]
+QED
 
 (*---------------------------------------------------------------------------*)
 (* In order to reason about Brzozowski, we use the following theorem.        *)
 (*---------------------------------------------------------------------------*)
 
-val Brzozowski_eqns = Q.store_thm
-("Brzozowski_eqns",
- `dom_Brz seen worklist acc ==>
-   (Brzozowski seen worklist acc =
-      case worklist
-       of [] => (seen,acc)
-       | r::t =>
-         if mem_regexp r seen then
-             Brzozowski seen t acc
-           else
-             let arcs = transitions r
-             in Brzozowski (insert_regexp r seen)
-                           (remove_dups (MAP SND arcs) ++ t)
-                           (build_table arcs r acc))`,
- rw_tac std_ss [Brzozowski_def]
-  >> CASE_TAC
-     >- rw [Brzozo_eqns]
-     >- (rw [Brzozo_eqns,LET_THM]
-          >> metis_tac [exec_Brz_equals_Brzozo,dom_Brz_eqns]));
-
+Theorem Brzozowski_eqns :
+ dom_Brz seen work acc
+  ==>
+ Brzozowski seen work acc =
+    if null work then
+        (seen,acc)
+    else let (m,t) = deleteFindMin work;
+                 r = FST m;
+         in if mem_regexp r seen then
+                Brzozowski seen t acc
+            else
+              let arcs = transitions r
+              in Brzozowski (insert_regexp r seen)
+                            (FOLDL (\work a. insert_regexp (SND a) work) t arcs)
+                            (build_table arcs r acc)
+Proof
+rw_tac std_ss [Brzozowski_def,LET_THM]
+ >- metis_tac [Brzozo_eqns]
+ >- (`?r x t. deleteFindMin work = ((r,x),t)` by metis_tac [ABS_PAIR_THM]
+      >> rw []
+      >> rw [SimpLHS, Once Brzozo_eqns]
+      >> (qpat_x_assum `dom_Brz seen work acc`
+              (mp_tac o SIMP_RULE list_ss [Once dom_Brz_eqns])
+          >> rw []))
+QED
 
 (*---------------------------------------------------------------------------*)
-(* Return to definition of compiler                                          *)
+(* Definitions that find the accept states and map the final results to      *)
+(* vector form.                                                              *)
 (*---------------------------------------------------------------------------*)
 
 Definition get_accepts_def :
@@ -645,17 +891,26 @@ Definition table_to_vectors_def:
          (mergesort (inv_image (\a b:num. a <= b) FST) table)
 End
 
+(*---------------------------------------------------------------------------*)
+(* The basic regexp compiler function                                        *)
+(*---------------------------------------------------------------------------*)
+
 Definition compile_regexp_def :
   compile_regexp r =
     let r' = normalize r ;
         (states,last_state,state_numbering,table)
-          = Brzozowski balanced_map$empty [r']
+          = Brzozowski balanced_map$empty
+                       (balanced_map$singleton r' ())
                        (1n, balanced_map$singleton r' 0n, []) ;
         delta_vecs = table_to_vectors table ;
         accepts_vec = accepts_to_vector (get_accepts state_numbering) last_state
     in
       (state_numbering, delta_vecs, accepts_vec)
 End
+
+(*---------------------------------------------------------------------------*)
+(* DFA evaluator                                                             *)
+(*---------------------------------------------------------------------------*)
 
 Definition exec_dfa_def :
  exec_dfa finals table n s =
@@ -679,113 +934,60 @@ Proof
    >- rw_tac list_ss [SimpLHS, Once exec_dfa_def]
 QED
 
-(*
-val exec_dfa_def =
-  Define
-   `(exec_dfa finals table n [] = EL n finals) /\
-    (exec_dfa finals table n (c::t) =
-        case EL (ORD c) (EL n table) of
-         | NONE => F
-         | SOME k => exec_dfa finals table k t)`;
-*)
+(*---------------------------------------------------------------------------*)
+(* Set of strings accepted by DFA generated from regexp r                    *)
+(*---------------------------------------------------------------------------*)
+
+Definition Brz_lang_def :
+  Brz_lang r =
+    let (state_map,table_vec,finals_vec) = compile_regexp r ;
+        tableV = fromList (MAP fromList table_vec) ;
+        finalsV = fromList finals_vec ;
+    in
+       exec_dfa finalsV tableV
+         (THE (lookup regexp_compare (normalize r) state_map))
+End
 
 
 (*---------------------------------------------------------------------------*)
-(* Returns a function of type :string -> bool                                *)
+(* Combines the DFA compilation and the DFA evaluator. Returns a function of *)
+(* type :string -> bool                                                      *)
 (*---------------------------------------------------------------------------*)
 
 Definition regexp_matcher_def :
  regexp_matcher r =
-    let (state_numbering,delta,accepts) = compile_regexp r ;
-        start_state = THE (balanced_map$lookup regexp_compare
-                               (normalize r) state_numbering) ;
-        acceptsV = fromList accepts;
-        deltaV = fromList (MAP fromList delta)
+    let (state_map,delta,accepts) = compile_regexp r ;
+        start_state = THE (lookup regexp_compare (normalize r) state_map) ;
+        acceptsV = fromList accepts ;
+        deltaV = fromList (MAP fromList delta) ;
     in
       exec_dfa acceptsV deltaV start_state
 End
 
-(*
-val regexp_matcher_def =
- Define
-  `regexp_matcher r =
-    let (state_numbering,delta,accepts) = compile_regexp r in
-    let start_state_opt =
-             balanced_map$lookup regexp_compare (normalize r) state_numbering
-    in
-      exec_dfa accepts delta (THE start_state_opt)`;
-*)
-
 (*---------------------------------------------------------------------------*)
-(* get_accepts properties                                                    *)
+(* Properties of get_accepts                                                 *)
 (*---------------------------------------------------------------------------*)
 
-val sorted_get_accepts = Q.store_thm
-("sorted_get_accepts",
- `!fmap. SORTED $<= (get_accepts fmap)`,
+Theorem sorted_get_accepts :
+  !fmap.
+     SORTED $<= (get_accepts fmap)
+Proof
  RW_TAC set_ss [get_accepts_def] THEN
  CONV_TAC (DEPTH_CONV ETA_CONV) THEN
  MATCH_MP_TAC mergesort_sorted THEN
- RW_TAC arith_ss [transitive_def, total_def]);
+ RW_TAC arith_ss [transitive_def, total_def]
+QED
 
-val lookup_bin = Q.prove
-(`!fmap fmap' n k v x.
-      (lookup cmp r (Bin n k v fmap fmap') = SOME x)
-      <=>
-      ((cmp r k = Equal) /\ (v = x)) \/
-      ((cmp r k = Less) /\ (lookup cmp r fmap = SOME x)) \/
-      ((cmp r k = Greater) /\ (lookup cmp r fmap' = SOME x))`,
- RW_TAC list_ss [lookup_def] THEN BasicProvers.CASE_TAC);
 
-val member_iff_lookup = Q.prove
-(`!fmap cmp x. member cmp x fmap <=> ?y. lookup cmp x fmap = SOME y`,
- Induct
-   >> rw_tac set_ss [member_def, lookup_def]
-   >> BasicProvers.EVERY_CASE_TAC);
-
-val member_bin = Q.prove
-(`!fmap fmap' n k v.
-     member cmp r (Bin n k v fmap fmap')
-      <=>
-      ((cmp r k = Equal) \/
-      ((cmp r k = Less) /\ member cmp r fmap) \/
-      ((cmp r k = Greater) /\ member cmp r fmap'))`,
- RW_TAC list_ss [member_def] THEN BasicProvers.CASE_TAC);
-
-val key_less_lookup = Q.prove
-(`!fmap cmp k1 k2 x.
-     invariant cmp fmap /\ good_cmp cmp /\
-     key_ordered cmp k1 fmap Less /\
-     (lookup cmp k2 fmap = SOME x)
-     ==>
-     (cmp k1 k2 = Less)`,
-Induct >> rw_tac list_ss [key_ordered_def, lookup_def, invariant_def]
-       >> every_case_tac
-          >- metis_tac []
-          >- metis_tac [good_cmp_def,comparison_distinct]
-          >- metis_tac []);
-
-val key_greater_lookup = Q.prove
-(`!fmap cmp k1 k2 x.
-     invariant cmp fmap /\ good_cmp cmp /\
-     key_ordered cmp k1 fmap Greater /\
-     (lookup cmp k2 fmap = SOME x)
-     ==>
-     (cmp k2 k1 = Less)`,
-Induct >> rw_tac list_ss [key_ordered_def, lookup_def, invariant_def]
-       >> every_case_tac
-          >- metis_tac []
-          >- metis_tac [good_cmp_def,comparison_distinct]
-          >- metis_tac []);
-
-val lemma = Q.prove
-(`!fmap x acc.
+Theorem mem_get_acceptsA[local] :
+ !fmap P x acc.
     balanced_map$invariant regexp_compare fmap /\
     MEM x (foldrWithKey
-               (\r n nlist. if nullable r then n::nlist else nlist)
+               (\r n nlist. if P r then n::nlist else nlist)
                acc fmap)
      ==>
-    MEM x acc \/ ?r. nullable r /\ (lookup regexp_compare r fmap = SOME x)`,
+    MEM x acc \/ ?r. P r /\ (lookup regexp_compare r fmap = SOME x)
+Proof
  Induct THEN RW_TAC std_ss []
   >- full_simp_tac list_ss [foldrWithKey_def,lookup_def]
   >- (simp_tac list_ss [lookup_bin]
@@ -803,46 +1005,51 @@ val lemma = Q.prove
         >- metis_tac [key_less_lookup,regexp_compare_good,good_cmp_thm]
         >- metis_tac [key_greater_lookup,regexp_compare_good,good_cmp_thm]
         >- metis_tac [key_less_lookup,regexp_compare_good,good_cmp_thm]
-        >- metis_tac [key_greater_lookup,regexp_compare_good,good_cmp_thm]));;
+        >- metis_tac [key_greater_lookup,regexp_compare_good,good_cmp_thm])
+QED
 
-val mem_acc = Q.prove
-(`!P fmap x acc.
+Theorem mem_foldrWithKey_mono[local] :
+ !P fmap x acc.
     MEM x acc
      ==>
      MEM x (foldrWithKey
                (\r n nlist. if P r then n::nlist else nlist)
-               acc fmap)`,
- gen_tac >> Induct >> RW_TAC std_ss [foldrWithKey_def] >> metis_tac [MEM]);
+               acc fmap)
+Proof
+  gen_tac
+   >> Induct
+   >> RW_TAC std_ss [foldrWithKey_def]
+   >> metis_tac [MEM]
+QED
 
-val lemma1 = Q.prove
-(`!P fmap r x acc.
+Theorem mem_get_acceptsB[local] :
+ !P fmap r x acc.
     P r /\ (lookup regexp_compare r fmap = SOME x)
      ==>
-     MEM x (foldrWithKey (\r n nlist. if P r then n::nlist else nlist) acc fmap)`,
- gen_tac >> Induct
- >- rw_tac list_ss [lookup_def,foldrWithKey_def]
- >- (rw_tac list_ss [lookup_bin,regexp_compare_eq,foldrWithKey_def]
-      >> metis_tac [mem_acc,MEM]));
+    MEM x (foldrWithKey (\r n nlist. if P r then n::nlist else nlist) acc fmap)
+Proof
+  gen_tac >> Induct
+  >- rw_tac list_ss [lookup_def,foldrWithKey_def]
+  >- (rw_tac list_ss [lookup_bin,regexp_compare_eq,foldrWithKey_def]
+       >> metis_tac [mem_foldrWithKey_mono,MEM])
+QED
 
-val mem_get_accepts = Q.store_thm
-("mem_get_accepts",
- `!bmap x.
-    invariant regexp_compare bmap ==>
-    (MEM x (get_accepts bmap)
+Theorem mem_get_accepts[local] :
+ !bmap x.
+    invariant regexp_compare bmap
+    ==>
+     (MEM x (get_accepts bmap)
        <=>
-     ?r. nullable r /\ (lookup regexp_compare r bmap = SOME x))`,
- rw_tac list_ss [get_accepts_def,mergesort_mem] >> metis_tac [lemma,lemma1,MEM]);
-
+      ?r. nullable r /\
+          (lookup regexp_compare r bmap = SOME x))
+Proof
+ rw_tac list_ss [get_accepts_def,mergesort_mem]
+  >> metis_tac [mem_get_acceptsA,mem_get_acceptsB,MEM]
+QED
 
 (*---------------------------------------------------------------------------*)
-(* Correctness of regexp compiler                                            *)
+(* Properties of extend_states                                               *)
 (*---------------------------------------------------------------------------*)
-
-Definition fmap_inj_def :
-  fmap_inj cmp bmap =
-     !x y. x IN fdom cmp bmap /\ (lookup cmp x bmap = lookup cmp y bmap)
-            ==> (cmp x y = Equal)
-End
 
 Definition extend_states_inv_def :
   extend_states_inv next_state state_map table =
@@ -852,19 +1059,22 @@ Definition extend_states_inv_def :
       (!n. MEM n (MAP SND table) ==> n < next_state))
 End
 
-val extend_states_inv = Q.prove (
-`!next_state state_map table states next_state' state_map' table'.
-  (extend_states next_state state_map table states = (next_state',state_map',table')) /\
-  extend_states_inv next_state state_map table
-  ==>
-  extend_states_inv next_state' state_map' table'`,
+Theorem extend_states_inv[local] :
+ !next_state state_map table states next_state' state_map' table'.
+     (extend_states next_state state_map table states
+         = (next_state',state_map',table')) /\
+     extend_states_inv next_state state_map table
+    ==>
+    extend_states_inv next_state' state_map' table'
+Proof
  ho_match_mp_tac extend_states_ind
   >> rw [extend_states_def]
   >> BasicProvers.EVERY_CASE_TAC
   >> fs []
   >> FIRST_X_ASSUM match_mp_tac
   >> rw []
-  >> fs [extend_states_inv_def, frange_def, MEM_MAP,EXTENSION,GSYM LEFT_FORALL_IMP_THM]
+  >> fs [extend_states_inv_def, frange_def,
+         MEM_MAP,EXTENSION,GSYM LEFT_FORALL_IMP_THM]
   >> `good_cmp regexp_compare /\ eq_cmp regexp_compare`
         by metis_tac [eq_cmp_regexp_compare,regexp_compare_good]
   >> rw_tac set_ss []
@@ -880,74 +1090,25 @@ val extend_states_inv = Q.prove (
   >- rw_tac set_ss []
   >- metis_tac [LESS_TRANS,DECIDE ``x < x+1n``,IN_DEF]
   >- (rw_tac set_ss [] >> metis_tac[])
-  >- metis_tac [LESS_TRANS,DECIDE ``x < x+1n``,IN_DEF])
+  >- metis_tac [LESS_TRANS,DECIDE ``x < x+1n``,IN_DEF]
+QED
 
-Definition submap_def :
-  submap cmp t1 t2 =
-     !x. x IN fdom cmp t1
-          ==> x IN fdom cmp t2 /\
-             (lookup cmp x t1 = lookup cmp x t2)
-End
 
-val submap_id = Q.prove
-(`!t cmp. submap cmp t t`,
- rw [submap_def]);
-
-val submap_trans = Q.prove
-(`!t1 t2 t3 cmp. submap cmp t1 t2 /\ submap cmp t2 t3 ==> submap cmp t1 t3`,
- rw [submap_def]);
-
-val submap_mono = Q.prove
-(`!t1 t2 k v cmp.
-    eq_cmp cmp /\ invariant cmp t2 /\ submap cmp t1 t2
-    /\ k NOTIN fdom cmp t1
+Theorem extend_states_thm :
+ !next_state state_map table states next_state' state_map' table'.
+    (extend_states next_state state_map table states
+       = (next_state',state_map',table')) /\
+    invariant regexp_compare state_map
    ==>
-   submap cmp t1 (insert cmp k v t2)`,
-  rw [submap_def,fdom_insert]
-  >> res_tac
-  >> `good_cmp cmp` by metis_tac [eq_cmp_def]
-  >> rw [lookup_insert_thm]
-  >> `k=x` by metis_tac [eq_cmp_def]
-  >> rw []
-  >> metis_tac[]);
-
-val submap_insert = Q.prove
-(`!bmap t cmp x v.
-    eq_cmp cmp /\ invariant cmp bmap /\
-    x NOTIN fdom cmp bmap /\
-    submap cmp (insert cmp x v bmap) t
-    ==> submap cmp bmap t`,
- rw_tac set_ss [submap_def]
-  >> `invariant cmp (insert cmp x v bmap)` by metis_tac [insert_thm,eq_cmp_def]
-  >- (qpat_x_assum `$! M` (mp_tac o Q.ID_SPEC) >> rw_tac set_ss [fdom_insert])
-  >- (`~(x' = x)` by (fs [fdom_def] >> metis_tac[])
-       >> `fdom cmp (insert cmp x v bmap) x'` by rw [fdom_insert,IN_DEF]
-       >> `good_cmp cmp` by metis_tac [eq_cmp_def]
-       >> `lookup cmp x' (insert cmp x v bmap) = lookup cmp x' t` by metis_tac[]
-       >> pop_assum (SUBST_ALL_TAC o SYM)
-       >> pat_elim `$!M`
-       >> rw_tac set_ss [lookup_insert_thm]
-       >> metis_tac [eq_cmp_def]));
-
-val set_lem = Q.prove
-(`!x s t. x IN s ==> (s UNION t = s UNION (x INSERT t))`,
- rw_tac set_ss [SET_EQ_THM] >> metis_tac []);
-
-Definition fapply_def :
-  fapply cmp bmap x = THE (lookup cmp x bmap)
-End
-
-val extend_states_thm = Q.prove
-(`!next_state state_map table states next_state' state_map' table'.
-  (extend_states next_state state_map table states = (next_state',state_map',table'))
-  /\ invariant regexp_compare state_map
-   ==>
-  (fdom regexp_compare state_map' = (fdom regexp_compare state_map UNION set (MAP SND states))) /\
+  (fdom regexp_compare state_map' =
+      (fdom regexp_compare state_map UNION set (MAP SND states))) /\
   submap regexp_compare state_map state_map' /\
   next_state <= next_state' /\
-  (table' = REVERSE (MAP (\(c,r). (c, fapply regexp_compare state_map' r)) states) ++ table) /\
-  invariant regexp_compare state_map'`
- ,
+  (table' = REVERSE
+             (MAP (\(c,r). (c, fapply regexp_compare state_map' r)) states)
+            ++ table) /\
+  invariant regexp_compare state_map'
+Proof
  `eq_cmp regexp_compare` by metis_tac [eq_cmp_regexp_compare]
   >> ho_match_mp_tac extend_states_ind
   >> rw [extend_states_def]
@@ -958,10 +1119,8 @@ val extend_states_thm = Q.prove
   >> res_tac
   >- (rw_tac set_ss [fdom_insert] >> metis_tac[])
   >- (`r' IN fdom regexp_compare state_map` by rw [fdom_def]
-       >> rw_tac set_ss [set_lem])
-  >- (match_mp_tac submap_insert
-      >> rw [fdom_def]
-      >> metis_tac [NOT_SOME_NONE])
+       >> rw_tac set_ss [IN_SET_UNION])
+  >- (match_mp_tac submap_insert >> rw [fdom_def] >> metis_tac [NOT_SOME_NONE])
   >- decide_tac
   >- (pat_elim `$! M` >> rw[]
        >> qpat_x_assum `submap _ __ ___` mp_tac
@@ -978,7 +1137,11 @@ val extend_states_thm = Q.prove
       >> pop_assum (mp_tac o Q.SPEC `r'`)
       >> rw [fdom_def]
       >> metis_tac [THE_DEF])
-);
+QED
+
+(*---------------------------------------------------------------------------*)
+(* What it means to be a good table                                          *)
+(*---------------------------------------------------------------------------*)
 
 Definition good_table_def :
   good_table state_map table =
@@ -997,6 +1160,10 @@ Definition good_table_def :
          (lookup regexp_compare r' state_map = SOME n') /\
          (r' = smart_deriv c r)))
 End
+
+(*---------------------------------------------------------------------------*)
+(* Some abbreviations                                                        *)
+(*---------------------------------------------------------------------------*)
 
 Definition invar_def : invar = invariant regexp_compare
 End
@@ -1019,265 +1186,88 @@ End
 Definition apply_def : apply = fapply regexp_compare
 End
 
+Definition set_of_def : set_of oset = fapply regexp_compare
+End
+
+Theorem dom_union[local] :
+ !a b.
+    invariant regexp_compare a /\ invariant regexp_compare b
+    ==>
+   (dom (union a b) = (dom a) UNION (dom b))
+Proof
+ metis_tac [regexp_compare_good,fdom_ounion,dom_def,union_def]
+QED
+
+(*---------------------------------------------------------------------------*)
+(* Invariants on regexp compilation                                          *)
+(*---------------------------------------------------------------------------*)
+
 Definition Brz_invariant_def :
  Brz_invariant seen todo (next_state,state_map,table) <=>
-    invar state_map /\ invar seen /\
-    EVERY is_normalized todo /\
+    invar todo /\ invar state_map /\ invar seen /\
+    (!r. oin regexp_compare r todo ==> is_normalized r) /\
     (!r. mem_regexp r seen ==> is_normalized r) /\
     (!r. r IN dom state_map ==> is_normalized r) /\
-    (dom (union seen (set todo)) = dom state_map) /\
+    (dom (union seen todo) = dom state_map) /\
     (range state_map = count next_state) /\
     (set (MAP FST table) = fdom num_cmp (oimage num_cmp (apply state_map) seen)) /\
     fmap_inj regexp_compare state_map /\
     good_table state_map table
 End
 
-val lem = Q.prove (
-`!b c d e f. Brz_invariant b c (d,e,f) ==> EVERY is_normalized c`,
- rw [Brz_invariant_def]);
+Theorem triv_lem[local] :
+  !s1 s2. (s1 = s2) ==> ((s1 UNION s) = (s2 UNION s))
+Proof
+ SET_TAC[]
+QED
 
-val fdom_ounion = Q.prove
-(`!a b. good_cmp cmp /\ invariant cmp a /\ invariant cmp b
-     ==> (fdom cmp (ounion cmp a b) = (fdom cmp a) UNION (fdom cmp b))`,
- rw[fdom_def,ounion_def,SET_EQ_THM]
-  >> metis_tac [regexp_compare_good,good_oset_def,
-       SIMP_RULE std_ss [oin_def,ounion_def,
-                         member_iff_lookup,oneTheory.one] oin_ounion]);
-
-val dom_union = Q.prove
-(`!a b. invariant regexp_compare a /\ invariant regexp_compare b
-        ==> (dom (union a b) = (dom a) UNION (dom b))`,
- metis_tac [regexp_compare_good,fdom_ounion,dom_def,union_def])
-
-val invariant_oset = Q.store_thm
-("invariant_oset",
- `!l. good_cmp cmp ==> invariant cmp (oset cmp l)`,
- simp_tac std_ss [oset_def]
-   >> Induct
-   >> fs [oempty_def,empty_def,oinsert_def]
-   >- metis_tac [invariant_def]
-   >- metis_tac [insert_thm]);
-
-val in_dom_oset = Q.store_thm
-("in_dom_oset",
- `!l x. eq_cmp cmp ==> (x IN fdom cmp (oset cmp l) <=> MEM x l)`,
- Induct >> rw []
-  >- rw [oempty_def,empty_def,fdom_def,lookup_def]
-  >- (`good_cmp cmp` by metis_tac [eq_cmp_def]
-       >> imp_res_tac invariant_oset >> pop_assum (assume_tac o Q.SPEC `l`)
-       >> rw [oset_def]
-       >> rw [GSYM oset_def]
-       >> rw [oinsert_def]
-       >> rw_tac set_ss [fdom_insert]));
-
-val dom_set_append = Q.store_thm
-("dom_set_append",
- `!l1 l2. dom (set (l1++l2)) = dom (set l1) UNION dom (set l2)`,
- rw[dom_def,set_def,EXTENSION] >>
- `eq_cmp regexp_compare` by metis_tac [eq_cmp_regexp_compare] >>
- rw [in_dom_oset]);
-
-val member_insert = Q.store_thm
-("member_insert",
- `!bmap x y v.
-    eq_cmp cmp /\ invariant cmp bmap ==>
-    (member cmp x (insert cmp y v bmap) <=> (x=y) \/ member cmp x bmap)`,
- rw [member_iff_lookup,GSYM (SIMP_RULE set_ss [SET_EQ_THM] fdom_def)] >>
- rw [fdom_insert] >> metis_tac [IN_DEF]);
-
-val triv_lem = Q.prove(`!s1 s2. (s1 = s2) ==> ((s1 UNION s) = (s2 UNION s))`,rw[]);
-
-val dom_oset_lem = Q.prove
-(`!l. eq_cmp cmp ==> (fdom cmp (oset cmp l) = LIST_TO_SET l)`,
- rw [EXTENSION,in_dom_oset,eq_cmp_regexp_compare]);
-
-val mem_foldrWithKey = Q.prove
-(`!(bset:'a oset) acc a. eq_cmp cmp /\ invariant cmp bset ==>
-     (MEM (a,()) (foldrWithKey (\k x xs. (k,())::xs) acc bset)
-            <=>
-      (a IN fdom cmp bset) \/ MEM (a,()) acc)`,
-simp_tac set_ss [fdom_def]
- >> Induct >> rw [foldrWithKey_def,invariant_def] >> fs []
- >- rw [lookup_def]
- >- (`good_cmp cmp` by metis_tac [eq_cmp_def]
-      >> rw [lookup_bin,EQ_IMP_THM]
-      >> metis_tac [key_greater_lookup,key_less_lookup,good_cmp_thm,eq_cmp_def]));
-
-val mem_foldrWithKey_lem =
-    mem_foldrWithKey
-      |> Q.SPEC `bset`
-      |> Q.SPEC `[]`
-      |> SIMP_RULE list_ss []
-
-val left_to_right = Q.prove
-(`eq_cmp cmp ==>
-   !list bmap k v. invariant cmp bmap /\
-        (lookup cmp k (FOLDR (\(k,v) t. insert cmp k v t) bmap list) = SOME v)
-            ==>
-           (MEM (k,v) list \/ (lookup cmp k bmap = SOME v))`,
- strip_tac
-  >> `good_cmp cmp` by metis_tac [eq_cmp_def]
-  >> Induct
-     >- rw []
-     >- (Cases_on `h` >> rw []
-          >> pop_assum mp_tac
-          >> `invariant cmp (FOLDR (\(k,v) t. insert cmp k v t) bmap list)`
-               by (Q.SPEC_TAC (`list`,`L`)
-                     >> Induct >> rw [invariant_def]
-                     >> Cases_on `h` >> rw [] >> metis_tac [insert_thm])
-          >> rw [lookup_insert_thm]
-          >> metis_tac [eq_cmp_def]));
-
-val invariant_ffoldr = Q.prove
-(`!list aset f.
-   good_cmp cmp /\ invariant cmp aset
+Theorem Brz_inv_pres[local] :
+ !todo1 x todos work seen next_state state_map table.
+    ~null work /\
+    (deleteFindMin work = ((todo1,x),todos)) /\
+    Brz_invariant seen work (next_state,state_map,table) /\
+    ~mem_regexp todo1 seen
    ==>
-   invariant cmp (FOLDR (\(k,v) t. insert cmp (f k) v t) aset list)`,
-  Induct >> rw [invariant_def]
-         >> Cases_on `h` >> rw [] >> metis_tac [insert_thm]);
-
-val invariant_ffoldr_inst =
-    invariant_ffoldr
-      |> INST_TYPE [beta |-> ``:unit``, gamma |-> beta]
-
-val left_to_right_alt = Q.prove
-(`eq_cmp (cmp:'b->'b->ordering)
-   ==>
-   !(list :('a # unit) list) (bset :'b oset) x f.
-      invariant cmp bset /\
-      (lookup cmp x (FOLDR (\(k,v:unit) t. insert cmp (f k) () t) bset list) = SOME ())
-            ==>
-           (?a. MEM (a,()) list /\ (x = f a))
-           \/
-           ((!a. MEM (a,()) list ==> (x <> f a)) /\ (lookup cmp x bset = SOME ()))`,
- strip_tac
-  >> `good_cmp cmp` by metis_tac [eq_cmp_def]
-  >> Induct
-     >- rw []
-     >- (Cases_on `h` >> rw [] >> fs []
-          >> pop_assum mp_tac
-          >> `invariant cmp (FOLDR (\(k,v:unit) t. insert cmp (f k) () t) bset list)`
-               by (Q.SPEC_TAC (`list`,`L`)
-                     >> Induct >> rw [invariant_def]
-                     >> Cases_on `h` >> rw [] >> metis_tac [insert_thm])
-          >> rw [lookup_insert_thm]
-          >> metis_tac [eq_cmp_def]));
-
-val left_to_right_lem =
-    left_to_right_alt
-      |> Q.GEN `cmp`
-      |> Q.SPEC `cmp2`
-      |> UNDISCH
-      |> Q.SPEC `foldrWithKey (\(k:'a) (x:unit) xs. (k,())::xs) [] aset`
-      |> Q.SPEC `Tip`
-      |> Q.SPEC `x`
-      |> Q.SPEC `f`
-      |> DISCH_ALL;
-
-val oin_fdom = Q.prove
-(`!aset x. oin cmp x aset <=> x IN fdom cmp aset`,
- rw [fdom_def, oin_def, member_iff_lookup]);
-
-val mem_oin = Q.prove
-(`!list x aset.
-     eq_cmp cmp /\ invariant cmp aset /\
-     MEM (x,()) list
-      ==>
-     oin cmp (f x) (FOLDR (\(k,u) s. insert cmp (f k) () s) aset list)`,
- Induct >> rw [oin_fdom]
-  >> `good_cmp cmp` by metis_tac [eq_cmp_def]
-  >> mp_tac (SPEC_ALL invariant_ffoldr_inst)
-  >| [all_tac, Cases_on `h`]
-  >> rw[fdom_insert]
-  >> metis_tac [oin_fdom,IN_DEF]);
-
-val mem_oin_inst =
-   mem_oin
-   |> SPEC_ALL
-   |> Q.INST [`cmp` |-> `cmp2`, `aset` |-> `Tip`, `x` |-> `x'`]
-   |> Q.GEN `list`
-
-val fdom_oimage = Q.store_thm
-("fdom_oimage",
- `!aset:'a oset.
-     eq_cmp (cmp1:'a->'a->ordering) /\
-     eq_cmp (cmp2:'b->'b->ordering) /\ invariant cmp1 aset
-    ==> (fdom cmp2 (oimage cmp2 f aset) = {f x | oin cmp1 x aset})`,
-simp_tac set_ss
-   [oimage_def,map_keys_def,balanced_mapTheory.fromList_def,fdom_def,
-    toAscList_def,empty_def,
-    rich_listTheory.FOLDR_MAP,LAMBDA_PROD,oneTheory.one]
- >> rw [EQ_IMP_THM]
-    >- (mp_tac left_to_right_lem >> rw[invariant_def]
-        >- (qexists_tac `a` >> rw[]
-             >> pat_elim `lookup _ __ ___ = SOME ()`
-             >> pat_elim `eq_cmp cmp2`
-             >> `a IN fdom cmp1 aset` by metis_tac [mem_foldrWithKey_lem]
-             >> pop_assum mp_tac
-             >> rw[oin_def,member_iff_lookup,fdom_def])
-        >- fs [lookup_def])
-    >- (`MEM (x',()) (foldrWithKey (\k x xs. (k,())::xs) [] aset)`
-          by metis_tac [oin_fdom,IN_DEF, mem_foldrWithKey_lem]
-         >> mp_tac mem_oin_inst >> rw [invariant_def]
-         >> res_tac
-         >> fs [oin_def,member_iff_lookup,oneTheory.one])
-);
-
-val fdom_oimage_rw =
- fdom_oimage
-   |> SIMP_RULE set_ss [GSPECIFICATION_applied];
-
-val fdom_oimage_insert = Q.prove
-(`!bset a f cmp1 cmp2.
-    eq_cmp (cmp1:'a->'a->ordering) /\
-     eq_cmp (cmp2:'b->'b->ordering) /\ invariant cmp1 bset
-         ==> (fdom cmp2 (oimage cmp2 f (oinsert cmp1 a bset))
-               =
-              ((f a) INSERT fdom cmp2 (oimage cmp2 f bset)))`,
-rpt strip_tac
- >> `invariant cmp1 (oinsert cmp1 a bset)` by metis_tac [insert_thm, eq_cmp_def,oinsert_def]
- >> mp_tac fdom_oimage_rw >> asm_simp_tac bool_ss[]
- >> rw_tac set_ss []
- >> `good_cmp cmp1 /\ good_cmp cmp2` by metis_tac [eq_cmp_def]
- >> rw [oin_def, member_iff_lookup, oinsert_def]
- >> fs [eq_cmp_def,lookup_insert_thm]
- >> metis_tac[]);
-
-
-val fdom_oimage_inst =
-   fdom_oimage
-   |> INST_TYPE [alpha |-> ``:regexp``, beta |-> ``:num``]
-   |> Q.INST [`cmp1` |-> `regexp_compare`, `cmp2` |-> `num_cmp`]
-   |> SIMP_RULE std_ss [eq_cmp_regexp_compare,num_cmp_good,num_cmp_antisym,eq_cmp_def]
-
-val Brz_inv_pres = Q.prove (
-`!todo1 todos seen next_state state_map table.
-  Brz_invariant seen (todo1::todos) (next_state,state_map,table) /\
-  ~mem_regexp todo1 seen
- ==>
-  Brz_invariant (insert_regexp todo1 seen)
-                (MAP SND (transitions todo1) ++ todos)
-                (build_table (transitions todo1)
-                             todo1 (next_state,state_map,table))`,
+   Brz_invariant (insert_regexp todo1 seen)
+                 (FOLDL (\work a. insert_regexp (SND a) work) todos (transitions todo1))
+                 (build_table (transitions todo1)
+                              todo1 (next_state,state_map,table))
+Proof
  rw_tac list_ss [good_table_def,insert_regexp_def, invar_def,
                  Brz_invariant_def, build_table_def, transitions_def,set_def] >>
- imp_res_tac extend_states_thm >>
- `todo1 IN dom state_map`
-   by (qpat_x_assum `dom (union a b) = dom state_map` (mp_tac o SYM) >> rw [] >>
-       `invariant regexp_compare
-         (oset regexp_compare (todo1::todos))` by metis_tac [invariant_oset,regexp_compare_good]
-       >> rw [dom_union]
-       >> disj2_tac
-       >> `eq_cmp regexp_compare` by metis_tac [eq_cmp_regexp_compare]
-       >> rw [dom_def,in_dom_oset])
-   >>
- `todo1 IN dom state_map'` by metis_tac [submap_def,dom_def]
- >>
- pop_assum (strip_assume_tac o SIMP_RULE set_ss [dom_def, fdom_def]) >> rw [] >>
-  rw [Brz_invariant_def, good_table_def,invar_def]
+ imp_res_tac extend_states_thm
+ >> `todo1 IN dom work`
+          by metis_tac [deleteFindMin_thm,EXTENSION,IN_UNION,IN_INSERT,dom_def]
+ >> `todo1 IN dom state_map` by metis_tac [dom_union,IN_UNION]
+ >> `todo1 IN dom state_map'` by metis_tac [submap_def,dom_def]
+ >> pop_assum (strip_assume_tac o SIMP_RULE set_ss [dom_def, fdom_def])
+ >> rw []
+ >> rw [Brz_invariant_def, good_table_def,invar_def]
+ (* 13 subgoals *)
+  >- metis_tac [deleteFindMin_thm,invariant_foldl]
   >- metis_tac [insert_thm,regexp_compare_good]
-  >- (rw [EVERY_MAP] >> Q.SPEC_TAC (`ALPHABET`,`alphabet`)
-       >> Induct >> rw [smart_deriv_normalized])
+  >- (`MEM r (MAP SND (MAP (\c. (c,smart_deriv c todo1)) ALPHABET)) \/
+       oin regexp_compare r todos`
+         by metis_tac [oin_foldl_insert,deleteFindMin_thm]
+       >- (fs [MEM_MAP,MAP_MAP_o,combinTheory.o_DEF]
+           >> match_mp_tac smart_deriv_normalized
+           >> `todo1 IN dom work`
+                  by metis_tac [deleteFindMin_thm,dom_def]
+           >> `oin regexp_compare todo1 work`
+                  by metis_tac [oin_fdom,dom_def]
+           >> metis_tac [])
+       >- (fs [oin_fdom]
+           >> `FDOM (to_fmap regexp_compare todos) =
+               FDOM (DRESTRICT (to_fmap regexp_compare work)
+                        (FDOM (to_fmap regexp_compare work) DELETE
+                                key_set regexp_compare todo1))`
+               by metis_tac [deleteFindMin,regexp_compare_good]
+           >> fs [FDOM_DRESTRICT,INTER_DELETE]
+           >> `{r} IN FDOM (to_fmap regexp_compare todos)`
+                 by metis_tac[SING_IN_FDOM,eq_cmp_regexp_compare,deleteFindMin_thm]
+           >> rfs[]
+           >> metis_tac [SING_IN_FDOM,eq_cmp_regexp_compare,deleteFindMin_thm])
+     )
   >- metis_tac [member_insert,mem_regexp_def,eq_cmp_regexp_compare,insert_thm,eq_cmp_def]
   >- (`r IN fdom regexp_compare state_map \/
        r IN set (MAP SND (MAP (\c. (c,smart_deriv c todo1)) ALPHABET))`
@@ -1288,22 +1278,28 @@ val Brz_inv_pres = Q.prove (
        >> rw [GSYM set_def]
        >> `invariant regexp_compare (insert regexp_compare todo1 () seen)`
             by metis_tac [insert_thm,regexp_compare_good]
-       >> `invariant regexp_compare
-             (set (MAP SND (MAP (\c. (c,smart_deriv c todo1)) ALPHABET) ++ todos))`
-           by metis_tac [invariant_oset, set_def,regexp_compare_good]
-       >> `invariant regexp_compare (set (todo1::todos))`
-          by metis_tac [invariant_oset, set_def, regexp_compare_good]
-       >> rw [dom_union]
-       >> rw_tac bool_ss [Once CONS_APPEND,dom_set_append]
        >> `dom (insert regexp_compare todo1 () seen) =
            dom (set [todo1]) UNION dom seen`
             by (rw [dom_def,fdom_insert,eq_cmp_regexp_compare,Once INSERT_SING_UNION]
                 >> match_mp_tac triv_lem
                 >> rw_tac bool_ss [EXTENSION,set_def]
-               >> rw [in_dom_oset,eq_cmp_regexp_compare])
-       >> rw []
-       >> rw [AC UNION_COMM UNION_ASSOC]
-       >> metis_tac [dom_oset_lem,eq_cmp_regexp_compare,dom_def,set_def])
+                >> rw [in_dom_oset,eq_cmp_regexp_compare])
+       >> `invariant regexp_compare
+             (FOLDL (\work' a. insert regexp_compare (SND a) () work') todos
+                (MAP (\c. (c,smart_deriv c todo1)) ALPHABET))`
+           by metis_tac [invariant_foldl,deleteFindMin_thm]
+       >> rw [dom_union]
+       >> rw [EXTENSION]
+       >> `invariant regexp_compare todos` by metis_tac [deleteFindMin_thm]
+       >> rw [oin_foldl_insert |> SIMP_RULE std_ss [oin_fdom,GSYM dom_def]]
+       >> rw [AC DISJ_COMM DISJ_ASSOC]
+       >> qsuff_tac `x IN dom work <=> (x IN dom (set [todo1]) \/ x IN dom todos)`
+           >- metis_tac[]
+       >> `dom work = {todo1} UNION dom todos`
+            by metis_tac [deleteFindMin_thm,dom_def]
+       >> qsuff_tac `{todo1} = dom (set [todo1])`
+           >- metis_tac[IN_UNION,EXTENSION]
+       >> simp_tac list_ss [dom_def,set_def,dom_oset_lem,eq_cmp_regexp_compare])
   >- (`extend_states_inv next_state state_map ([]:(num,num) alist)`
                by (rw [extend_states_inv_def] >> metis_tac [range_def])
        >> imp_res_tac extend_states_inv
@@ -1312,17 +1308,17 @@ val Brz_inv_pres = Q.prove (
       >> `eq_cmp num_cmp /\ eq_cmp regexp_compare`
             by metis_tac[eq_cmp_regexp_compare,num_cmp_good,num_cmp_antisym,eq_cmp_def]
       >> rw [GSYM oinsert_def,fdom_oimage_insert]
-      >> `apply state_map' todo1 = x` by rw [apply_def,fapply_def]
+      >> `apply state_map' todo1 = x'` by rw [apply_def,fapply_def]
       >> pop_assum SUBST_ALL_TAC
       >> AP_TERM_TAC
       >> `dom seen SUBSET dom state_map` by
            (qpat_x_assum `dom _ = dom state_map` (SUBST_ALL_TAC o SYM)
              >> metis_tac [invariant_oset, eq_cmp_def,dom_union,SUBSET_UNION])
       >> rw[fdom_oimage_inst,SET_EQ_THM,EQ_IMP_THM,oin_fdom]
-      >> Q.EXISTS_TAC `x''` >> rw[]
-      >> `x'' IN dom state_map` by metis_tac [SUBSET_DEF,dom_def]
-      >> `(x'' IN dom state_map') /\
-          (lookup regexp_compare x'' state_map = lookup regexp_compare x'' state_map')`
+      >> Q.EXISTS_TAC `x'''` >> rw[]
+      >> `x''' IN dom state_map` by metis_tac [SUBSET_DEF,dom_def]
+      >> `(x''' IN dom state_map') /\
+          (lookup regexp_compare x''' state_map = lookup regexp_compare x''' state_map')`
            by metis_tac [submap_def,dom_def]
       >> rw [apply_def,fapply_def])
   >- (`extend_states_inv next_state state_map ([]:(num,num) alist)`
@@ -1347,14 +1343,14 @@ val Brz_inv_pres = Q.prove (
              >> metis_tac [invariant_oset, eq_cmp_def,dom_union,SUBSET_UNION])
        >> pop_assum mp_tac
        >> rw_tac set_ss [dom_def, fdom_def, member_iff_lookup,SUBSET_DEF,oneTheory.one]
-       >> Q.EXISTS_TAC `x'` >> rw[]
+       >> Q.EXISTS_TAC `x''` >> rw[]
        >> strip_tac
-       >> `x' IN fdom regexp_compare state_map` by fs [SUBSET_DEF,dom_def, fdom_def]
-       >> `(x' IN fdom regexp_compare state_map') /\
-           (lookup regexp_compare x' state_map = lookup regexp_compare x' state_map')`
+       >> `x'' IN fdom regexp_compare state_map` by fs [SUBSET_DEF,dom_def, fdom_def]
+       >> `(x'' IN fdom regexp_compare state_map') /\
+           (lookup regexp_compare x'' state_map = lookup regexp_compare x'' state_map')`
              by (fs [submap_def,fdom_def, member_iff_lookup] >> metis_tac [])
        >> fs []
-       >> `x' <> todo1` by (fs[mem_regexp_def,member_iff_lookup] >> metis_tac[])
+       >> `x'' <> todo1` by (fs[mem_regexp_def,member_iff_lookup] >> metis_tac[])
        >> metis_tac [fmap_inj_def,eq_cmp_regexp_compare, eq_cmp_def])
   >- (pop_assum mp_tac
         >> rw[MAP_MAP_o,combinTheory.o_DEF]
@@ -1378,139 +1374,173 @@ val Brz_inv_pres = Q.prove (
                            >> metis_tac [IN_DEF])
                   >> fs [fdom_def, member_iff_lookup])
            >- (fs[submap_def, fdom_def, member_iff_lookup] >> metis_tac[]))
-);
+QED
 
-
-val Brz_invariant_alt = Q.prove
-(`!seen worklist worklist' acc.
-   (LIST_TO_SET worklist = LIST_TO_SET worklist')
-   ==>
-   (Brz_invariant seen worklist acc = Brz_invariant seen worklist' acc)`,
-rpt strip_tac >> PairCases_on `acc`
- >> rw[Brz_invariant_def,EQ_IMP_THM]
- >> ((qpat_x_assum `EVERY _ __` mp_tac >>
-        qpat_x_assum `LIST_TO_SET _ = LIST_TO_SET __` mp_tac
-         >> rw [EVERY_MEM]
-         >> NO_TAC)
-    ORELSE
-     (qpat_x_assum `dom _ = dom __` (SUBST_ALL_TAC o SYM)
-         >> fs [invar_def]
-         >> `invariant regexp_compare (set worklist') /\
-             invariant regexp_compare (set worklist)`
-              by metis_tac [invariant_oset,set_def, regexp_compare_good]
-         >> rw [dom_union,EXTENSION]
-         >> `eq_cmp regexp_compare` by metis_tac [eq_cmp_regexp_compare]
-         >> rw [in_dom_oset,dom_def,set_def])));
-
-val Brz_inv_thm = Q.prove
-(`!seen worklist acc.
-   dom_Brz seen worklist acc
+Theorem Brz_inv_thm[local] :
+ !seen work acc.
+   dom_Brz seen work acc
    ==>
     !seen' acc'.
-      Brz_invariant seen worklist acc /\
-      (Brzozowski seen worklist acc = (seen',acc'))
+      Brz_invariant seen work acc /\
+      (Brzozowski seen work acc = (seen',acc'))
       ==>
-       Brz_invariant seen' [] acc'`,
- ho_match_mp_tac Brzozowski_ind
-   >> rw []
-   >> qpat_x_assum `Brzozowski _ __ ___ = _4` mp_tac
-   >> rw [Brzozowski_eqns]
-   >> pop_assum mp_tac
-   >> CASE_TAC
-   >> rw[]
-      >- metis_tac[]
-      >- (rfs []
-          >> first_assum match_mp_tac
-          >> qpat_x_assum `Brz_invariant seen (h::t) args` mp_tac
-          >> PairCases_on `acc`
-          >> rw [Brz_invariant_def]
-          >> qpat_x_assum `dom _ = dom __` (SUBST_ALL_TAC o SYM)
-          >> fs [invar_def]
-          >> `invariant regexp_compare (set t) /\
-              invariant regexp_compare (set (h::t))`
-              by metis_tac [invariant_oset,set_def, regexp_compare_good]
-          >> rw [dom_union,EXTENSION]
-          >> `eq_cmp regexp_compare` by metis_tac [eq_cmp_regexp_compare]
-          >> rw [in_dom_oset,dom_def,set_def]
-          >> fs [mem_regexp_def, member_iff_lookup]
-          >> rw [fdom_def]
-          >> metis_tac[])
-      >- (rfs [LET_THM]
-          >> rw[]
-          >> pat_elim `_ = __`
-          >> PairCases_on `acc`
-          >> imp_res_tac Brz_inv_pres
-          >> `LIST_TO_SET (remove_dups (MAP SND (transitions h)) ++ t) =
-              LIST_TO_SET (MAP SND (transitions h) ++ t)`
-                    by rw [EXTENSION,remove_dups_mem]
-          >> metis_tac [Brz_invariant_alt]))
+       Brz_invariant seen' balanced_map$empty acc'
+Proof
+ simp_tac std_ss [empty_def]
+ >> ho_match_mp_tac Brzozowski_ind
+ >> rw []
+ >> qpat_x_assum `Brzozowski _ __ ___ = _4` mp_tac
+ >> rw [Brzozowski_eqns]
+    >- (Cases_on `work` >> fs[null_def])
+    >- (`?r work'. deleteFindMin work = ((r,()),work')`
+            by metis_tac [ABS_PAIR_THM,oneTheory.one]
+        >> fs[]
+        >> BasicProvers.NORM_TAC set_ss []
+        >> first_x_assum match_mp_tac
+        >> rw[]
+        >- (qpat_x_assum `Brz_invariant _ _ _` mp_tac
+            >> `?next_state state_map table.
+                  acc = (next_state,state_map,table)` by metis_tac[ABS_PAIR_THM]
+            >> pop_assum subst_all_tac
+            >> rw [Brz_invariant_def]
+               >- metis_tac [deleteFindMin_thm,invar_def]
+               >- metis_tac[deleteFindMin_thm,invar_def,
+                            oin_fdom,IN_UNION,IN_INSERT,EXTENSION]
+               >- (qpat_x_assum `dom (union seen work) = dom state_map`
+                                (subst_all_tac o SYM)
+                   >> fs [invar_def,dom_def,union_def, mem_regexp_def,GSYM oin_def]
+                   >> `invariant regexp_compare work' /\
+                       fdom regexp_compare work =
+                       {r} UNION fdom regexp_compare work'`
+                       by metis_tac[deleteFindMin_thm,invar_def]
+                   >> fs [GSYM oin_fdom,EXTENSION,oin_ounion,good_oset_def,
+                          regexp_compare_good]
+                   >> metis_tac[]))
+        >- metis_tac [Brz_inv_pres,ABS_PAIR_THM])
+QED
 
-val Brz_mono = Q.prove
-(`!seen worklist acc.
-  dom_Brz seen worklist acc
-  ==>
-  !seen' acc'.
-    Brz_invariant seen worklist acc /\
-    (Brzozowski seen worklist acc = (seen',acc'))
-  ==>
-    submap regexp_compare (FST (SND acc)) (FST(SND acc'))`,
+
+Theorem Brz_mono[local] :
+ !seen work acc.
+   dom_Brz seen work acc
+   ==>
+   !seen' acc'.
+     Brz_invariant seen work acc /\
+     (Brzozowski seen work acc = (seen',acc'))
+     ==>
+     submap regexp_compare (FST (SND acc)) (FST(SND acc'))
+Proof
  ho_match_mp_tac Brzozowski_ind
- >> Cases_on `worklist`
-    >- (rw []
-         >> qpat_x_assum `Brzozowski _ __ ___ = _4` mp_tac
-         >> rw [Brzozowski_eqns,submap_id])
-    >- (rw []
-         >> qpat_x_assum `Brzozowski _ __ ___ = _4` mp_tac
-         >> rw [Brzozowski_eqns]
-         >> fs[LET_THM]
-            >- (first_assum match_mp_tac
-                >> qpat_x_assum `Brz_invariant seen (h::t) acc` mp_tac
-                >> PairCases_on `acc`
-                >> rw [Brz_invariant_def]
-                >> qpat_x_assum `dom _ = dom __` (SUBST_ALL_TAC o SYM)
-                >> fs [invar_def]
-                >> `invariant regexp_compare (set t) /\
-                    invariant regexp_compare (set (h::t))`
-                      by metis_tac [invariant_oset,set_def, regexp_compare_good]
-                >> rw [dom_union,EXTENSION]
-                >> `eq_cmp regexp_compare` by metis_tac [eq_cmp_regexp_compare]
-                >> rw [in_dom_oset,dom_def,set_def]
-                >> fs [mem_regexp_def, member_iff_lookup]
-                >> rw [fdom_def]
+ >> rw[]
+ >> qpat_x_assum `Brzozowski _ __ ___ = _4` mp_tac
+ >> rw [Brzozowski_eqns]
+ >> fs []
+  >- metis_tac [submap_id]
+  >- (`?r work'. deleteFindMin work = ((r,()),work')`
+            by metis_tac [ABS_PAIR_THM,oneTheory.one]
+      >> fs[]
+      >> BasicProvers.NORM_TAC set_ss []
+       >- (first_assum match_mp_tac
+           >> qexists_tac `seen'` >> rw[]
+           >> qpat_x_assum `Brz_invariant seen work acc` mp_tac
+           >> `?next_state state_map table.
+                     acc = (next_state,state_map,table)` by metis_tac[ABS_PAIR_THM]
+           >> pop_assum subst_all_tac
+           >> rw [Brz_invariant_def,invar_def]
+            >- metis_tac [deleteFindMin_thm]
+            >- metis_tac[deleteFindMin_thm,invar_def,
+                         oin_fdom,IN_UNION,IN_INSERT,EXTENSION]
+            >- (qpat_x_assum `dom (union seen work) = dom state_map`
+                             (subst_all_tac o SYM)
+                >> fs [invar_def,dom_def,union_def,
+                       mem_regexp_def,GSYM oin_def]
+                >> `invariant regexp_compare work' /\
+                    fdom regexp_compare work =
+                    {r} UNION fdom regexp_compare work'`
+                          by metis_tac[deleteFindMin_thm,invar_def]
+                >> fs [GSYM oin_fdom,EXTENSION,oin_ounion,
+                       good_oset_def,regexp_compare_good]
                 >> metis_tac[])
-            >- (rw[]
-                >> pat_elim `_ = __`
-                >> PairCases_on `acc`
-                >> imp_res_tac Brz_inv_pres
-                >> `LIST_TO_SET (remove_dups (MAP SND (transitions h)) ++ t) =
-                    LIST_TO_SET (MAP SND (transitions h) ++ t)`
-                        by rw [EXTENSION,remove_dups_mem]
-                >> imp_res_tac Brz_invariant_alt
-                >> fs[]
-                >> NTAC 3 (pop_assum (K ALL_TAC))
-                >> match_mp_tac submap_trans
-                >> qexists_tac `FST (SND (build_table (transitions h) h (acc0,acc1,acc2)))`
-                >> rw[build_table_def,LET_THM]
-                >> `?x state_map'' z. extend_states acc0 acc1 [] (transitions h) = (x,state_map'',z)`
-                       by metis_tac [pair_CASES]
-                >> fs[]
-                >> `invariant regexp_compare acc1`
-                     by metis_tac [Brz_invariant_def, invar_def]
-                >> imp_res_tac extend_states_thm
-                >> rw []
-                >> CASE_TAC
-                >> fs []
-                >> match_mp_tac submap_mono
-                >> rw[eq_cmp_regexp_compare]
-                >> qpat_x_assum `submap _ __ ___` mp_tac
-                >> rw [submap_def]
-                >> strip_tac
-                >> res_tac
-                >> fs [fdom_def]
-                >> metis_tac [NOT_SOME_NONE])));
+          )
+       >- (`?next_state state_map table.
+               acc = (next_state,state_map,table)` by metis_tac[ABS_PAIR_THM]
+           >> pop_assum subst_all_tac
+           >> imp_res_tac Brz_inv_pres
+           >> fs []
+           >> match_mp_tac submap_trans
+           >> qexists_tac
+              `FST (SND (build_table (transitions r) r
+                                     (next_state,state_map,table)))`
+           >> fs[]
+           >> rw[build_table_def,LET_THM]
+           >> `?next_state' state_map' trans'.
+                 extend_states next_state state_map [] (transitions r)
+                  = (next_state',state_map', trans')`
+                by metis_tac[ABS_PAIR_THM]
+           >> rw[]
+           >> `invariant regexp_compare state_map` by metis_tac [Brz_invariant_def,invar_def]
+           >> imp_res_tac extend_states_thm
+           >> CASE_TAC
+           >> rw[]
+           >> match_mp_tac submap_mono
+           >> rw[eq_cmp_regexp_compare]
+           >> strip_tac
+           >> `r IN fdom regexp_compare state_map'` by metis_tac[submap_def]
+           >> pop_assum mp_tac
+           >> simp_tac set_ss [fdom_def]
+           >> metis_tac[NOT_SOME_NONE]))
+QED
+
+Theorem Brz_invariant_final[local] :
+ !seen next_state state_map table.
+   Brz_invariant seen empty (next_state,state_map,table)
+    ==>
+    (next_state = LENGTH table) /\
+    PERM (MAP FST table) (COUNT_LIST (LENGTH table)) /\
+    (!x. MEM x (get_accepts state_map) ==> x < LENGTH table) /\
+    (!n l c. (ALOOKUP table n = SOME l) /\ (?x. ALOOKUP l c = SOME x) ==> MEM c ALPHABET)
+Proof
+ simp [Brz_invariant_def,invar_def,set_def,ounion_oempty,union_def] >>
+ rpt gen_tac >> strip_tac >> conj_asm1_tac
+ >- (`!x. x IN set (MAP FST table) ==> x < next_state`
+           by (fs [count_def, EXTENSION, range_def, frange_def,dom_def]
+                >> rw [fdom_oimage_inst,apply_def,oin_fdom]
+                >> fs [fdom_def,fapply_def]
+                >> metis_tac [THE_DEF,ounion_oempty,oempty_def])
+     >>
+     `LENGTH table = CARD (set (MAP FST table))`
+           by metis_tac [LENGTH_MAP,ALL_DISTINCT_CARD_LIST_TO_SET, good_table_def]
+     >>
+     `fdom num_cmp (oimage num_cmp (apply state_map) seen) = range state_map`
+       by (simp_tac set_ss [range_def, frange_def] >>
+           qpat_x_assum `dom _ = dom __` mp_tac >>
+           rw [fdom_oimage_inst,apply_def, oin_fdom,fapply_def, dom_def] >>
+           fs[fdom_def,ounion_oempty, GSYM oempty_def,EXTENSION] >>
+           metis_tac[THE_DEF])
+     >> rw [])
+ >> conj_asm1_tac
+   >- (match_mp_tac PERM_ALL_DISTINCT
+       >> rw [all_distinct_count_list, MEM_COUNT_LIST]
+        >- fs [good_table_def]
+        >- (`fdom num_cmp (oimage num_cmp (apply state_map) seen) = range state_map`
+             by (simp_tac set_ss [range_def, frange_def] >>
+                 qpat_x_assum `dom _ = dom __` mp_tac >>
+                 simp_tac set_ss [ounion_oempty, GSYM oempty_def] >>
+                 rw [fdom_oimage_inst,apply_def, oin_fdom,fapply_def, dom_def] >>
+                 fs [fdom_def,EXTENSION] >> metis_tac[THE_DEF])
+            >> qpat_x_assum `set (MAP FST table) = _` (subst_all_tac o SYM)
+            >> rw[]))
+ >> conj_tac
+ >- (rw [mem_get_accepts]
+     >> `x IN range state_map`
+           by (simp_tac set_ss [range_def, frange_def] >> metis_tac[])
+     >> rfs [count_def])
+ >- (rw [] >> fs [good_table_def] >> metis_tac [])
+QED
+
 
 (*---------------------------------------------------------------------------*)
-(* table_lang                                                                *)
+(* table_lang parallels the definition of exec_dfa                           *)
 (*---------------------------------------------------------------------------*)
 
 Definition table_lang_def :
@@ -1524,18 +1554,19 @@ Definition table_lang_def :
              | SOME n' => table_lang final_states table n' t)
 End
 
-val table_lang_correct = Q.prove
-(`!finals table state_map.
-  fmap_inj regexp_compare state_map /\
-  good_table state_map table /\
-  (set (MAP FST table) = frange regexp_compare state_map) /\
-  (!n r. (lookup regexp_compare r state_map = SOME n) ==> (MEM n finals <=> nullable r))
-  ==>
-  !n r s.
-    (!c. MEM c s ==> MEM c ALPHABET) /\
-    (lookup regexp_compare r state_map = SOME n)
-    ==>
-    (table_lang finals table n s <=> smart_deriv_matches r (MAP CHR s))`,
+Theorem table_lang_correct[local] :
+ !finals table state_map.
+   fmap_inj regexp_compare state_map /\
+   good_table state_map table /\
+   (set (MAP FST table) = frange regexp_compare state_map) /\
+   (!n r. (lookup regexp_compare r state_map = SOME n) ==> (MEM n finals <=> nullable r))
+   ==>
+   !n r s.
+     (!c. MEM c s ==> MEM c ALPHABET) /\
+     (lookup regexp_compare r state_map = SOME n)
+     ==>
+     (table_lang finals table n s <=> smart_deriv_matches r (MAP CHR s))
+Proof
  rpt gen_tac >>
  strip_tac >>
  Induct_on `s` >>
@@ -1559,72 +1590,67 @@ val table_lang_correct = Q.prove
          by (qpat_x_assum `fmap_inj _ __` mp_tac
               >> rw_tac set_ss [fmap_inj_def,fdom_def,regexp_compare_eq])
      >> rw []
-     >> metis_tac [ORD_CHR_lem,mem_alphabet]))
+     >> metis_tac [ORD_CHR_lem,mem_alphabet])
+QED
 
-val vec_lang_lem1 = Q.prove
-(`!(n:num). MEM n finals_list <=>
-           (ALOOKUP (MAP (\x. (x,T)) finals_list) n = SOME T)`,
+Theorem vec_lang_lem1[local] :
+ !(n:num).
+    MEM n finals_list <=> (ALOOKUP (MAP (\x. (x,T)) finals_list) n = SOME T)
+Proof
  rw [EQ_IMP_THM]
   >- rw [alistTheory.ALOOKUP_TABULATE]
   >- (`MEM (n,T) (MAP (\x. (x,T)) finals_list)` by METIS_TAC [alistTheory.ALOOKUP_MEM]
-      >> fs[MEM_MAP]));
+      >> fs[MEM_MAP])
+QED
 
-val vec_lang_lem2 =
+Theorem vec_lang_lem2 =
   alistTheory.alookup_stable_sorted
      |> Q.INST_TYPE [`:'a` |-> `:num`, `:'b` |-> `:(num, 'a) alist`]
      |> Q.SPECL [`$<=`, `mergesort`, `n`, `table`]
      |> SIMP_RULE (srw_ss()++ARITH_ss) [transitive_def, total_def, mergesort_STABLE_SORT];
 
-(* Following are a bit suss because of use of ORD *)
-val vec_lang_lem3 =
+Theorem vec_lang_lem3 =
   alistTheory.alookup_stable_sorted
      |> Q.INST_TYPE [`:'a` |-> `:num`, `:'b` |-> `:'a option`]
      |> Q.SPECL [`$<=`, `mergesort`, `n`, `MAP (\(c,n). (c,SOME n)) table2`]
      |> SIMP_RULE (srw_ss()++ARITH_ss)
            [transitive_def, total_def, mergesort_STABLE_SORT, stringTheory.char_le_def];
 
-val vec_lang_lem4 = Q.prove (
-`!l x. ALOOKUP (MAP (\(c,n). (c,SOME n)) l) x =
-       OPTION_MAP SOME (ALOOKUP l x)`,
+Theorem vec_lang_lem4[local] :
+ !l x. ALOOKUP (MAP (\(c,n). (c,SOME n)) l) x = OPTION_MAP SOME (ALOOKUP l x)
+Proof
  Induct_on `l` >>
  rw [] >>
  PairCases_on `h` >>
  rw [] >>
- fs [stringTheory.ORD_11]);
+ fs [stringTheory.ORD_11]
+QED
 
-val leq_thm =
- let val leq = numSyntax.leq_tm
- in Q.prove (`transitive ^leq /\ total ^leq /\ antisymmetric ^leq`,
-    srw_tac [ARITH_ss] [transitive_def, total_def, antisymmetric_def])
- end;
 
-val length_mergesort = Q.prove
-(`!l R. LENGTH (mergesort R l) = LENGTH l`,
- metis_tac[mergesort_perm,PERM_LENGTH]);
-
-val table_to_vec_thm = Q.prove (
-`!table final_states max_char max_state table' final_states'.
-  (max_char = alphabet_size) /\
-  SORTED $<= final_states /\
-  (!x. MEM x final_states ==> x < max_state) /\
-  (!n l c. (ALOOKUP table n = SOME l) /\ (?x. ALOOKUP l c = SOME x) ==> c < max_char) /\
-  PERM (MAP FST table) (COUNT_LIST (LENGTH table)) /\
-  (table_to_vectors table = table') /\
-  (accepts_to_vector final_states max_state = final_states')
+Theorem table_to_vec_thm[local] :
+ !table final_states max_char max_state table' final_states'.
+    (max_char = alphabet_size) /\
+    SORTED $<= final_states /\
+    (!x. MEM x final_states ==> x < max_state) /\
+    (!n l c. (ALOOKUP table n = SOME l) /\
+             (?x. ALOOKUP l c = SOME x) ==> c < max_char) /\
+    PERM (MAP FST table) (COUNT_LIST (LENGTH table)) /\
+    (table_to_vectors table = table') /\
+    (accepts_to_vector final_states max_state = final_states')
   ==>
-  (LENGTH table' = LENGTH table) /\
-  (LENGTH final_states' = max_state) /\
-  (!n. MEM n final_states <=> n < LENGTH final_states' /\ EL n final_states') /\
-  (!n. (?l. ALOOKUP table n = SOME l) <=> n < LENGTH table') /\
-  (!n l. n < LENGTH table' ==> (LENGTH (EL n table') = max_char)) /\
-  (!n c x.
-    (?l. (ALOOKUP table n = SOME l) /\ (ALOOKUP l c = SOME x)) <=>
-    n < LENGTH table' /\ c < LENGTH (EL n table') /\ (EL c (EL n table') = SOME x))`
- ,
+   (LENGTH table' = LENGTH table) /\
+   (LENGTH final_states' = max_state) /\
+   (!n. MEM n final_states <=> n < LENGTH final_states' /\ EL n final_states') /\
+   (!n. (?l. ALOOKUP table n = SOME l) <=> n < LENGTH table') /\
+   (!n l. n < LENGTH table' ==> (LENGTH (EL n table') = max_char)) /\
+   (!n c x.
+     (?l. (ALOOKUP table n = SOME l) /\ (ALOOKUP l c = SOME x)) <=>
+     n < LENGTH table' /\
+     c < LENGTH (EL n table') /\ (EL c (EL n table') = SOME x))
+Proof
  simp [good_table_def, table_to_vectors_def,accepts_to_vector_def] >>
  rpt gen_tac >>
  strip_tac >>
-(* `FINITE final_states` by metis_tac [finite_bounded] >> *)
  qabbrev_tac `sorted_table = mergesort (inv_image $<= FST) table` >>
  `LENGTH sorted_table = LENGTH table` by metis_tac [mergesort_perm, PERM_LENGTH] >>
  `SORTS mergesort (inv_image $<= (FST : num # (num,'a) alist -> num))`
@@ -1666,7 +1692,8 @@ val table_to_vec_thm = Q.prove (
          fs [MEM_MAP, MEM_COUNT_LIST] >>
          metis_tac [FST,mergesort_perm,PERM_LENGTH])
      >- (`ALOOKUP sorted_table n = SOME (EL n (MAP SND sorted_table))`
-                by metis_tac [dense_alist_to_vec_thm, LENGTH_COUNT_LIST,mergesort_perm,PERM_LENGTH] >>
+             by metis_tac [dense_alist_to_vec_thm,
+                   LENGTH_COUNT_LIST,mergesort_perm,PERM_LENGTH] >>
          `ALOOKUP table n = SOME (EL n (MAP SND sorted_table))`
                 by metis_tac [vec_lang_lem2] >>
          rw [])) >>
@@ -1677,37 +1704,29 @@ val table_to_vec_thm = Q.prove (
  simp [EL_MAP,length_mergesort] >>
  conj_tac
  >- (rw [] >>
-     `?n' table2'. EL n sorted_table = (n',table2')` by metis_tac [pair_CASES] >>
-     rw [] >>
+     `?n' table2'. EL n sorted_table = (n',table2')`
+          by metis_tac [pair_CASES] >> rw [] >>
      qabbrev_tac `sorted_table2 =
-                  mergesort (inv_image $<= FST) (MAP (\(c,n). (c,SOME n)) table2')` >>
+         mergesort (inv_image $<= FST) (MAP (\(c,n). (c,SOME n)) table2')` >>
      qabbrev_tac `table2 = EL n (MAP SND sorted_table)` >>
      `SORTED $<= (MAP FST sorted_table2)`
-             by (fs [SORTS_DEF, sorted_map, leq_thm] >>
-                 metis_tac []) >>
+             by (fs [SORTS_DEF, sorted_map, leq_thm] >> metis_tac []) >>
      metis_tac [alist_to_vec_thm])
  >- (* last conjunct *)
  (fs [length_mergesort] >>
-  rw [] >>  eq_tac >>  strip_tac >>
-  res_tac >>
- simp [EL_MAP] >>
+  rw [] >>  eq_tac >>  strip_tac >> res_tac >> simp [EL_MAP] >>
  `?n' table2'. EL n sorted_table = (n',table2')` by metis_tac [pair_CASES] >>
  rw [] >>
  qabbrev_tac `sorted_table2 =
-              mergesort (inv_image $<= FST) (MAP (\(c,n). (c,SOME n)) table2')` >>
+      mergesort (inv_image $<= FST) (MAP (\(c,n). (c,SOME n)) table2')` >>
  qabbrev_tac `table2 = EL n (MAP SND sorted_table)` >>
  `SORTED $<= (MAP FST sorted_table2)`
-         by (fs [SORTS_DEF, sorted_map, leq_thm] >>
-             metis_tac [])
+         by (fs [SORTS_DEF, sorted_map, leq_thm] >> metis_tac [])
  >- metis_tac [alist_to_vec_thm]
  >- (imp_res_tac alist_to_vec_thm >>
      fs [AND_IMP_INTRO] >>
-     FIRST_X_ASSUM match_mp_tac >>
-     rw [] >>
-     `table2' = table2`
-            by (UNABBREV_ALL_TAC >>
-                rw [EL_MAP]) >>
-     rw [] >>
+     FIRST_X_ASSUM match_mp_tac >>  rw [] >>
+     `table2' = table2` by (UNABBREV_ALL_TAC >> rw [EL_MAP]) >> rw [] >>
      `ALOOKUP sorted_table n = SOME (EL n (MAP SND sorted_table))`
                 by metis_tac [dense_alist_to_vec_thm, LENGTH_COUNT_LIST] >>
      `ALOOKUP table n = SOME (EL n (MAP SND sorted_table))`
@@ -1719,15 +1738,11 @@ val table_to_vec_thm = Q.prove (
      fs [Once (GSYM vec_lang_lem3)] >>
      metis_tac [NOT_SOME_NONE, alist_to_vec_thm])
  >- (REV_FULL_SIMP_TAC std_ss [EL_MAP] >>
-     `table2' = table2`
-                by (UNABBREV_ALL_TAC >>
-                    rw [EL_MAP]) >>
-     fs [] >>
-     res_tac >>
-     simp [] >>
+     `table2' = table2` by (UNABBREV_ALL_TAC >> rw [EL_MAP]) >> fs [] >>
+     res_tac >> simp [] >>
      Cases_on `ALOOKUP sorted_table2 c`
      >- (`ALOOKUP (MAP (\(c,n). (c,SOME n)) table2) c = NONE`
-                 by metis_tac [vec_lang_lem4, OPTION_MAP_DEF, vec_lang_lem3] >>
+          by metis_tac [vec_lang_lem4, OPTION_MAP_DEF, vec_lang_lem3] >>
          metis_tac [NOT_SOME_NONE, alist_to_vec_thm])
     >- (`ALOOKUP sorted_table n = SOME (EL n (MAP SND sorted_table))`
            by metis_tac [dense_alist_to_vec_thm, LENGTH_COUNT_LIST] >>
@@ -1740,51 +1755,12 @@ val table_to_vec_thm = Q.prove (
         qunabbrev_tac `sorted_table2` >>
         fs [Once vec_lang_lem3] >>
         fs [vec_lang_lem4])))
-);
+QED
 
 
-val Brz_invariant_final = Q.prove (
-`!seen next_state state_map table.
-  Brz_invariant seen [] (next_state,state_map,table)
-  ==>
-  (next_state = LENGTH table) /\
-  PERM (MAP FST table) (COUNT_LIST (LENGTH table)) /\
-  (!x. MEM x (get_accepts state_map) ==> x < LENGTH table) /\
-  (!n l c. (ALOOKUP table n = SOME l) /\ (?x. ALOOKUP l c = SOME x) ==> MEM c ALPHABET)`
- ,
- simp [Brz_invariant_def,invar_def,set_def,ounion_oempty,union_def] >>
- rpt gen_tac >> strip_tac >>
- conj_asm1_tac
- >- (`!x. x IN set (MAP FST table) ==> x < next_state`
-           by (fs [count_def, EXTENSION, range_def, frange_def,dom_def]
-                >> rw [fdom_oimage_inst,apply_def,oin_fdom]
-                >> fs [fdom_def,fapply_def]
-                >> metis_tac [THE_DEF]) >>
-     `LENGTH table = CARD (set (MAP FST table))`
-           by metis_tac [LENGTH_MAP,ALL_DISTINCT_CARD_LIST_TO_SET, good_table_def] >>
-     `fdom num_cmp (oimage num_cmp (apply state_map) seen) = range state_map`
-       by (simp_tac set_ss [range_def, frange_def] >>
-           qpat_x_assum `dom _ = dom __` mp_tac >>
-           rw [fdom_oimage_inst,apply_def, oin_fdom,fapply_def, dom_def] >>
-           simp_tac set_ss [fdom_def] >> metis_tac[THE_DEF])
-     >> rw [])
->> conj_asm1_tac
-    >- (match_mp_tac PERM_ALL_DISTINCT
-          >> rw [all_distinct_count_list, MEM_COUNT_LIST]
-              >- fs [good_table_def]
-              >- (`fdom num_cmp (oimage num_cmp (apply state_map) seen) = range state_map`
-                    by (simp_tac set_ss [range_def, frange_def] >>
-                        qpat_x_assum `dom _ = dom __` mp_tac >>
-                        rw [fdom_oimage_inst,apply_def, oin_fdom,fapply_def, dom_def] >>
-                        simp_tac set_ss [fdom_def] >> metis_tac[THE_DEF])
-                    >> rw[]))
->> conj_tac
-   >- (rw [mem_get_accepts]
-      >> `x IN range state_map`
-            by (simp_tac set_ss [range_def, frange_def] >> metis_tac[])
-      >> rfs [count_def] )
-   >- (rw [] >> fs [good_table_def] >> metis_tac [])
-);
+(*---------------------------------------------------------------------------*)
+(* Well-formedness of final state vector                                     *)
+(*---------------------------------------------------------------------------*)
 
 Definition good_vec_def :
  good_vec vec final_states
@@ -1796,21 +1772,22 @@ Definition good_vec_def :
     (LENGTH final_states = LENGTH vec)
 End
 
-val Brz_inv_to_good_vec = Q.prove
-(`!seen next_state state_map table.
- Brz_invariant seen [] (next_state,state_map,table) /\
-  (table_to_vectors table = vec) /\
-  (accepts_to_vector (get_accepts state_map) next_state = final_states)
-  ==>
-  (next_state = LENGTH table) /\
-  good_vec vec final_states /\
-  (!r n. (lookup regexp_compare r state_map = SOME n) ==> n < LENGTH vec)`
- ,
+
+Theorem Brz_inv_to_good_vec[local] :
+ !seen next_state state_map table.
+   Brz_invariant seen empty (next_state,state_map,table) /\
+    (table_to_vectors table = vec) /\
+    (accepts_to_vector (get_accepts state_map) next_state = final_states)
+    ==>
+    (next_state = LENGTH table) /\
+    good_vec vec final_states /\
+    (!r n. (lookup regexp_compare r state_map = SOME n) ==> n < LENGTH vec)
+Proof
  simp [good_vec_def]
   >> rpt gen_tac >> strip_tac
   >> imp_res_tac Brz_invariant_final
   >> fs [Brz_invariant_def,invar_def,
-        ounion_oempty,union_def, set_def, oset_def]
+        ounion_oempty,GSYM oempty_def,union_def, set_def, oset_def]
   >>
   `(LENGTH vec = LENGTH table) /\
    (LENGTH final_states = LENGTH table) /\
@@ -1838,80 +1815,30 @@ val Brz_inv_to_good_vec = Q.prove
         by metis_tac [MEM_PERM,MEM_COUNT_LIST]
        >> rw [fdom_oimage_inst,apply_def, oin_fdom,fapply_def,SYM dom_def]
        >> simp_tac set_ss [dom_def,fdom_def, member_iff_lookup]
-       >> metis_tac [THE_DEF]));
-
-val compile_regexp_good_vec = Q.store_thm
-("compile_regexp_good_vec",
-`!r state_map table final_states.
-  dom_Brz empty [normalize r] (1,singleton (normalize r) 0,[]) /\
-  (compile_regexp r = (state_map, table, final_states))
-  ==>
-  good_vec table final_states /\
-  (!r n. (lookup regexp_compare r state_map = SOME n) ==> n < LENGTH table) /\
-  normalize r IN fdom regexp_compare state_map`
- ,
- simp [compile_regexp_def]
-  >> rpt gen_tac >> strip_tac
-  >> fs []
-  >> `?seen next_state state_map table.
-         Brzozowski empty [normalize r] (1,singleton (normalize r) 0,[])
-          = (seen,next_state,state_map,table)`
-       by metis_tac [pair_CASES]
-  >> fs []
-  >> `Brz_invariant empty [normalize r] (1,singleton (normalize r) 0,[])`
-     by
-      (fs [Brz_invariant_def,invar_def,dom_def, normalize_thm, fmap_inj_def, good_table_def,
-          singleton_thm,empty_def,invariant_def,mem_regexp_def,member_iff_lookup]
-        >> rw [lookup_def]
-           >- (fs [fdom_def, singleton_def,lookup_def]
-                >> BasicProvers.EVERY_CASE_TAC
-                >> rw []
-                >> metis_tac [eq_cmp_regexp_compare, eq_cmp_def,normalize_thm])
-           >- (rw [union_def,set_def,GSYM empty_def, GSYM oempty_def] >>
-               rw [EXTENSION,fdom_def, osingleton_def, singleton_def, lookup_def] >>
-               CASE_TAC)
-           >- (rw [range_def,frange_def, EXTENSION, singleton_def,lookup_def,EQ_IMP_THM]
-                >- (BasicProvers.EVERY_CASE_TAC >> rw [])
-                >- (Q.EXISTS_TAC `normalize r` >> rw [regexp_compare_id] >> decide_tac))
-           >- (rw [GSYM empty_def, GSYM oempty_def]
-               >> rw [fdom_def, lookup_def, empty_def, oempty_def])
-           >- (ntac 2 (pop_assum mp_tac)
-                >> simp_tac set_ss [fdom_def,singleton_def,lookup_def]
-                >> BasicProvers.EVERY_CASE_TAC
-                >> rw[]
-                >> metis_tac [eq_cmp_def, eq_cmp_regexp_compare]))
- >> imp_res_tac Brz_inv_thm
- >> imp_res_tac Brz_mono
- >> imp_res_tac Brz_inv_to_good_vec
- >> fs []
- >> rw []
-    >- metis_tac []
-    >- (`normalize r IN fdom regexp_compare (singleton (normalize r) 0)`
-         by rw [submap_def,fdom_def,singleton_def,lookup_def,regexp_compare_id]
-         >> metis_tac [submap_def])
-);
+       >> metis_tac [THE_DEF])
+QED
 
 
-val vec_lang_correct = Q.prove
-(`!table final_states max_char vec final_states'.
-  (max_char = alphabet_size) /\
-  SORTED $<= final_states /\
-  (!x. MEM x final_states ==> x < LENGTH table) /\
-  (!n l c. (ALOOKUP table n = SOME l) /\ (?x. ALOOKUP l c = SOME x) ==> c < max_char) /\
-  (PERM (MAP FST table) (COUNT_LIST (LENGTH table))) /\
-  (!n'. n' IN BIGUNION (IMAGE alist_range (alist_range table)) ==> n' < LENGTH table) /\
-  (table_to_vectors table = vec) /\
-  (accepts_to_vector final_states (LENGTH table) = final_states')
-  ==>
-  !n s. (!c. MEM c s ==> c < max_char) /\ n < LENGTH table
-       ==>
+Theorem vec_lang_correct :
+ !table final_states max_char vec final_states'.
+   (max_char = alphabet_size) /\
+   SORTED $<= final_states /\
+   (!x. MEM x final_states ==> x < LENGTH table) /\
+   (!n l c. (ALOOKUP table n = SOME l) /\ (?x. ALOOKUP l c = SOME x) ==> c < max_char) /\
+   (PERM (MAP FST table) (COUNT_LIST (LENGTH table))) /\
+   (!n'. n' IN BIGUNION (IMAGE alist_range (alist_range table)) ==> n' < LENGTH table) /\
+   (table_to_vectors table = vec) /\
+   (accepts_to_vector final_states (LENGTH table) = final_states')
+   ==>
+   !n s. (!c. MEM c s ==> c < max_char) /\ n < LENGTH table
+         ==>
         (table_lang final_states table n s
            <=>
          exec_dfa (fromList final_states')
                   (fromList (MAP fromList vec))
                   n
-                  (MAP CHR s))`
- ,
+                  (MAP CHR s))
+Proof
  rpt gen_tac
   >> strip_tac
   >> `(LENGTH vec = LENGTH table) /\
@@ -1950,50 +1877,41 @@ val vec_lang_correct = Q.prove
           >> rw [PULL_EXISTS]
           >> rw [alistTheory.alist_range_def, EXTENSION]
           >> metis_tac [])
-);
+QED
 
 
-Definition Brz_lang_def :
-  Brz_lang r =
-    let (state_map,table_vec,finals_vec) = compile_regexp r ;
-        tableV = fromList (MAP fromList table_vec) ;
-        finalsV = fromList finals_vec;
-    in
-       exec_dfa finalsV tableV (apply state_map (normalize r))
-End
+(*---------------------------------------------------------------------------*)
+(* Main correctness theorem: strings accepted by DFA are just the strings    *)
+(* specified by regexp r                                                     *)
+(*---------------------------------------------------------------------------*)
 
-val string_to_numlist = Q.prove
-(`!s. (!c. c IN set s ==> ORD c IN set ALPHABET) ==>
-      ?nl. (s = MAP CHR nl) /\ (!n. n IN set nl ==> n IN set ALPHABET)`,
- Induct >> rw []
-  >> `?nl. (s = MAP CHR nl) /\ !n. MEM n nl ==> MEM n ALPHABET` by metis_tac[]
-  >> `?n. (h = CHR n) /\ n < 256` by metis_tac [CHR_ONTO]
-  >> Q.EXISTS_TAC `n::nl`
-  >> rw []
-  >> metis_tac [ORD_CHR_RWT,alphabet_size_def]);
-
-
-val Brzozowski_correct = Q.store_thm
-("Brzozowski_correct",
-`!r s.
-  dom_Brz empty [normalize r] (1,singleton (normalize r) 0,[]) /\
-  (!c. MEM c s ==> MEM (ORD c) ALPHABET)
-  ==>
-  (Brz_lang r s = regexp_lang (normalize r) s)`
- ,
+Theorem Brzozowski_correct :
+ !r s.
+   dom_Brz empty (singleton (normalize r) ())
+           (1,singleton (normalize r) 0,[]) /\
+   (!c. MEM c s ==> MEM (ORD c) ALPHABET)
+   ==>
+   (Brz_lang r s = regexp_lang (normalize r) s)
+Proof
  rw [GSYM regexp_lang_smart_deriv, Brz_lang_def]
   >> UNABBREV_ALL_TAC
   >> fs [compile_regexp_def]
   >> `?seen next_state state_map table.
-        Brzozowski empty [normalize r] (1,singleton (normalize r) 0,[])
-          = (seen,next_state,state_map,table)`
+        Brzozowski empty (singleton (normalize r) ())
+                  (1,singleton (normalize r) 0,[]) = (seen,next_state,state_map,table)`
        by metis_tac [pair_CASES,SND]
   >> fs [LET_THM]
   >> rw []
-  >> `Brz_invariant empty [normalize r] (1,singleton (normalize r) 0,[])`
+  >> `Brz_invariant empty (singleton (normalize r) ())
+                   (1,singleton (normalize r) 0,[])`
       by (rw_tac set_ss [Brz_invariant_def,invar_def,dom_def, normalize_thm,
                       fmap_inj_def, good_table_def, singleton_thm,empty_def,
                       invariant_def,mem_regexp_def,member_iff_lookup]
+           >- (fs[singleton_def,oin_def,member_def]
+                >> BasicProvers.EVERY_CASE_TAC
+                >- metis_tac[]
+                >- metis_tac[eq_cmp_regexp_compare,eq_cmp_def,normalize_thm]
+                >- metis_tac[])
            >- fs [lookup_def]
            >- (fs [fdom_def, singleton_def,lookup_def]
                 >> BasicProvers.EVERY_CASE_TAC
@@ -2023,10 +1941,12 @@ val Brzozowski_correct = Q.store_thm
       <=>
      table_lang (get_accepts state_map) table (apply state_map (normalize r)) (MAP ORD s)`
      by (fs [invar_def,set_def,ounion_oempty,union_def]
-          >> `fdom num_cmp (oimage num_cmp (apply state_map) seen) = frange regexp_compare state_map`
+          >> `fdom num_cmp (oimage num_cmp (apply state_map) seen)
+               = frange regexp_compare state_map`
                     by (simp_tac set_ss [frange_def] >>
                         qpat_x_assum `dom _ = dom __` mp_tac >>
                         rw [fdom_oimage_inst,apply_def, oin_fdom,fapply_def, dom_def] >>
+                        fs[ounion_oempty, GSYM oempty_def] >>
                         simp_tac set_ss [fdom_def] >> metis_tac[THE_DEF])
           >> mp_tac (table_lang_correct
                    |> INST_TYPE [alpha |-> ``:num``]
@@ -2098,72 +2018,69 @@ val Brzozowski_correct = Q.store_thm
                     >> fs [regexp_compare_id])
         >> `0n IN count (LENGTH table)` by metis_tac [EXTENSION]
         >> metis_tac [IN_COUNT])
-);
+QED
 
-val Brzozowski_correct_again = Q.store_thm
-("Brzozowski_correct",
-`!r s.
-  dom_Brz empty [normalize r] (1,singleton (normalize r) 0,[]) /\
-  (!c. MEM c s ==> MEM (ORD c) ALPHABET)
-  ==>
-  (regexp_matcher r s = regexp_lang r s)`
- ,
+Theorem Brzozowski_correct_alt :
+ !r s.
+    dom_Brz empty (singleton (normalize r) ())
+            (1,singleton (normalize r) 0,[]) /\
+    (!c. MEM c s ==> MEM (ORD c) ALPHABET)
+   ==>
+   (regexp_matcher r s = regexp_lang r s)
+Proof
  rw []
   >> `Brz_lang r s = regexp_lang r s`
       by metis_tac [regexp_lang_normalize,Brzozowski_correct]
   >> pop_assum (SUBST_ALL_TAC o SYM)
-  >> rw [Brz_lang_def, regexp_matcher_def, LET_THM,apply_def,fapply_def]);
+  >> rw [Brz_lang_def, regexp_matcher_def, LET_THM,apply_def,fapply_def]
+QED
 
-val Brzozowski_partial_eval = Q.store_thm
-("Brzozowski_partial_eval",
-`!r state_numbering delta accepts deltaV acceptsV start_state.
-  (compile_regexp r = (state_numbering,delta,accepts)) /\
-  (deltaV = fromList (MAP fromList delta)) /\
-  (acceptsV = fromList accepts) /\
-  (lookup regexp_compare (normalize r) state_numbering = SOME start_state) /\
-  dom_Brz empty [normalize r] (1,singleton (normalize r) 0,[])
-  ==> !s. EVERY (\c. MEM (ORD c) ALPHABET) s
-          ==>
-         (exec_dfa acceptsV deltaV start_state s = regexp_lang r s)`
- ,
+Theorem Brzozowski_partial_eval :
+ !r state_numbering delta accepts deltaV acceptsV start_state.
+    (compile_regexp r = (state_numbering,delta,accepts)) /\
+    (deltaV = fromList (MAP fromList delta)) /\
+    (acceptsV = fromList accepts) /\
+    (lookup regexp_compare (normalize r) state_numbering = SOME start_state) /\
+    dom_Brz empty (singleton (normalize r) ())
+                  (1,singleton (normalize r) 0,[])
+    ==>
+    !s. EVERY (\c. MEM (ORD c) ALPHABET) s
+    ==>
+    (exec_dfa acceptsV deltaV start_state s = regexp_lang r s)
+Proof
  rw [EVERY_MEM]
   >> `regexp_matcher r s = regexp_lang r s`
-      by metis_tac [Brzozowski_correct_again]
+      by metis_tac [Brzozowski_correct_alt]
   >> pop_assum (SUBST_ALL_TAC o SYM)
-  >> rw [regexp_matcher_def, LET_THM]);
+  >> rw [regexp_matcher_def, LET_THM]
+QED
 
-val all_ord_string = Q.prove
-(`EVERY (\c. MEM (ORD c) ALPHABET) s
-   <=>
-  EVERY (\c. ORD c < alphabet_size) s`,
- simp_tac list_ss [mem_alphabet_iff]);
 
-val Brzozowski_partial_eval_conseq = Q.store_thm
-("Brzozowski_partial_eval_conseq",
- `!r state_numbering delta accepts deltaV acceptsV start_state.
-  (compile_regexp r = (state_numbering,delta,accepts)) /\
-  (deltaV = fromList (MAP fromList delta)) /\
-  (acceptsV = fromList accepts) /\
-  (lookup regexp_compare (normalize r) state_numbering = SOME start_state) /\
-  dom_Brz_alt empty [normalize r]
-  ==>
-  !s. EVERY (\c. ORD c < alphabet_size) s
-      ==>
-      (exec_dfa acceptsV deltaV start_state s = regexp_lang r s)`
- ,
- metis_tac[Brzozowski_partial_eval,all_ord_string,dom_Brz_alt_equal,all_ord_string]);
-
+Theorem Brzozowski_partial_eval_conseq :
+ !r state_numbering delta accepts deltaV acceptsV start_state.
+    (compile_regexp r = (state_numbering,delta,accepts)) /\
+    (deltaV = fromList (MAP fromList delta)) /\
+    (acceptsV = fromList accepts) /\
+    (lookup regexp_compare (normalize r) state_numbering = SOME start_state) /\
+    dom_Brz_alt empty (singleton (normalize r) ())
+    ==>
+    !s. EVERY (\c. ORD c < alphabet_size) s
+    ==>
+    (exec_dfa acceptsV deltaV start_state s = regexp_lang r s)
+Proof
+ metis_tac[Brzozowski_partial_eval,all_ord_string,
+           dom_Brz_alt_equal,all_ord_string]
+QED
 
 (*---------------------------------------------------------------------------*)
 (* Eliminate check that all chars in string are in alphabet. This can be     *)
 (* be done when alphabet = [0..255]                                          *)
 (*---------------------------------------------------------------------------*)
 
-val Brzozowski_partial_eval_256 = save_thm
-("Brzozowski_partial_eval_256",
+Theorem Brzozowski_partial_eval_256 =
   if Regexp_Type.alphabet_size = 256 then
    SIMP_RULE list_ss [ORD_BOUND,alphabet_size_def] Brzozowski_partial_eval_conseq
-  else TRUTH);
+  else TRUTH;
 
 
 (* val _ = EmitTeX.tex_theory"-"; *)
