examples/formal-languages/regular/vec_mapScript.sml
@@ -10,12 +10,11 @@ val _ = temp_tight_equality ();
 
 val every_case_tac = BasicProvers.EVERY_CASE_TAC;
 
-val alist_to_vec_def =
- Define
-  `(alist_to_vec l default 0 max = []) ∧
-   (alist_to_vec [] default (SUC n) max = default :: alist_to_vec [] default n max) ∧
-   (alist_to_vec ((x,y)::t) default (SUC n) max =
-    if SUC n ≤ max then
+Definition alist_to_vec_def :
+  (alist_to_vec l default 0 max = []) /\
+  (alist_to_vec [] default (SUC n) max = default :: alist_to_vec [] default n max) /\
+  (alist_to_vec ((x,y)::t) default (SUC n) max =
+    if SUC n <= max then
        if x = max - SUC n then
           y :: alist_to_vec t default n max
        else if x < max - SUC n then
@@ -23,19 +22,21 @@ val alist_to_vec_def =
        else
          default :: alist_to_vec ((x,y)::t) default n max
     else
-      [])`;
+      [])
+End
 
 val alist_to_vec_ind = fetch "-" "alist_to_vec_ind";
 
-val alist_to_vec_correct = Q.prove (
-`!l default cur max v.
-  SORTED $<= (MAP FST l) ∧
-  cur ≤ max ∧
+Theorem alist_to_vec_correct[local] :
+ !l default cur max v.
+  SORTED $<= (MAP FST l) /\
+  cur <= max /\
   alist_to_vec l default cur max = v
-  ⇒
-  LENGTH v = cur ∧
-  (!n x. n < cur ∧ ALOOKUP l (max - cur + n) = SOME x ⇒ EL n v = x) ∧
-  (!n. n < cur ∧ ALOOKUP l (max - cur + n) = NONE ⇒  EL n v = default)`,
+  ==>
+  LENGTH v = cur /\
+  (!n x. n < cur /\ ALOOKUP l (max - cur + n) = SOME x ==> EL n v = x) /\
+  (!n. n < cur /\ ALOOKUP l (max - cur + n) = NONE ==>  EL n v = default)
+Proof
  ho_match_mp_tac alist_to_vec_ind
  >> rw [alist_to_vec_def]
  >> `transitive $<=` by srw_tac [ARITH_ss] [transitive_def]
@@ -43,46 +44,49 @@ val alist_to_vec_correct = Q.prove (
  >> full_simp_tac (srw_ss()++ARITH_ss) [SORTED_EQ]
  >> Cases_on `n` >> rw [EL_CONS] >> fs []
     >- (FIRST_X_ASSUM match_mp_tac >> rw []
-        >> `max − SUC cur <> max + SUC n' − SUC cur` by decide_tac
-        >> `max + SUC n' - SUC cur = max + n' − cur` by decide_tac
+        >> `max - SUC cur <> max + SUC n' - SUC cur` by decide_tac
+        >> `max + SUC n' - SUC cur = max + n' - cur` by decide_tac
         >> metis_tac[])
     >- (FIRST_X_ASSUM match_mp_tac >> rw []
-        >> `max − SUC cur <> max + SUC n' − SUC cur` by decide_tac
-        >> `max + SUC n' - SUC cur = max + n' − cur` by decide_tac
+        >> `max - SUC cur <> max + SUC n' - SUC cur` by decide_tac
+        >> `max + SUC n' - SUC cur = max + n' - cur` by decide_tac
         >> metis_tac[])
     >- (ntac 2 (pop_assum mp_tac) >> rw []
         >> imp_res_tac ALOOKUP_MEM
-        >> `MEM (max − SUC cur) (MAP FST l)` by (rw[MEM_MAP] >> metis_tac[FST])
+        >> `MEM (max - SUC cur) (MAP FST l)` by (rw[MEM_MAP] >> metis_tac[FST])
         >> res_tac
         >> full_simp_tac (srw_ss()++ARITH_ss) [])
     >- (FIRST_X_ASSUM match_mp_tac >> rw []
         >> full_simp_tac (srw_ss()++ARITH_ss) []
-        >> `max + SUC n' − SUC cur  = max + n' − cur` by decide_tac
+        >> `max + SUC n' - SUC cur  = max + n' - cur` by decide_tac
         >> metis_tac[])
     >- (FIRST_X_ASSUM match_mp_tac >> rw []
         >> full_simp_tac (srw_ss()++ARITH_ss) []
-        >> `max + SUC n' − SUC cur = max + n' − cur` by decide_tac
+        >> `max + SUC n' - SUC cur = max + n' - cur` by decide_tac
         >> metis_tac[])
-);
+QED
 
-val alist_to_vec_thm = Q.store_thm ("alist_to_vec_thm",
-`!l default max v.
-  SORTED $<= (MAP FST l) ∧
+Theorem alist_to_vec_thm :
+ !l default max v.
+  SORTED $<= (MAP FST l) /\
   alist_to_vec l default max max = v
-  ⇒
-  LENGTH v = max ∧
-  (!n x. n < max ∧ ALOOKUP l n = SOME x ⇒ EL n v = x) ∧
-  (!n. n < max ∧ ALOOKUP l n = NONE ⇒  EL n v = default)`,
+  ==>
+  LENGTH v = max /\
+  (!n x. n < max /\ ALOOKUP l n = SOME x ==> EL n v = x) /\
+  (!n. n < max /\ ALOOKUP l n = NONE ==>  EL n v = default)
+Proof
  rw [] >>
  imp_res_tac alist_to_vec_correct >>
- fs []);
+ fs []
+QED
 
-val dense_alist_to_vec_correct = Q.prove (
-`!y l n.
-  MAP FST l = MAP (\x. x + y) (COUNT_LIST (LENGTH l)) ∧
+Theorem dense_alist_to_vec_correct[local] :
+ !y l n.
+  MAP FST l = MAP (\x. x + y) (COUNT_LIST (LENGTH l)) /\
   n < LENGTH l
-  ⇒
-  ALOOKUP l (n + y) = SOME (EL n (MAP SND l))`,
+  ==>
+  ALOOKUP l (n + y) = SOME (EL n (MAP SND l))
+Proof
  Induct_on `n` >>
  rw [] >>
  Cases_on `l` >>
@@ -95,13 +99,15 @@ val dense_alist_to_vec_correct = Q.prove (
  FIRST_X_ASSUM (mp_tac o Q.SPECL [`SUC h0`,`t`]) >>
  rw [] >>
  `!h0 x. h0 + SUC x = x + SUC h0` by decide_tac >>
- full_simp_tac bool_ss []);
+ full_simp_tac bool_ss []
+QED
 
-val dense_alist_to_vec_thm = Q.store_thm
-("dense_alist_to_vec_thm",
- `!l n. MAP FST l = COUNT_LIST (LENGTH l) ∧ n < LENGTH l
-        ⇒
-       ALOOKUP l n = SOME (EL n (MAP SND l))`,
- metis_tac [SIMP_RULE (srw_ss()) [] (Q.SPEC `0` dense_alist_to_vec_correct)]);
+Theorem dense_alist_to_vec_thm :
+ !l n. MAP FST l = COUNT_LIST (LENGTH l) /\ n < LENGTH l
+        ==>
+       ALOOKUP l n = SOME (EL n (MAP SND l))
+Proof
+ metis_tac [SIMP_RULE (srw_ss()) [] (Q.SPEC `0` dense_alist_to_vec_correct)]
+QED
 
 val _ = export_theory ();
